horror module adjusting + examples renaming + some refactoring

lam_cl_es_no.v
@@ -4,10 +4,11 @@ Require Import refocusing_lang.
 Require Import reduction_semantics_facts.
 
 
+
 Open Scope list.
 
 
-Module no_es_cl_ECCa <: RED_LANG.
+Module Lam_ClES_NO_PreLang <: RED_SYNTAX.
 
   Require Export Peano_dec Compare_dec.
 
@@ -25,7 +26,7 @@ Module no_es_cl_ECCa <: RED_LANG.
   | Sub   : closure -> substitut
   | Shift : nat     -> substitut.
 
-  Notation env    := (list (nat * substitut)).
+  Notation env     := (list (nat * substitut)).
   Notation "t @ s" := (Cl t s) (at level 10).
 
 
@@ -54,7 +55,13 @@ Module no_es_cl_ECCa <: RED_LANG.
   Definition ckind := ck.
   Hint Unfold ckind.
 
-  Definition CECa (k : ckind) := match k with CBot => False | _ => True end.
+
+  Definition CECa  (k : ckind) := match k with CBot => False | _ => True end.
+
+  Ltac destruct_all_CECa :=
+      repeat match goal with H : CECa ?k |- _ => 
+          try destruct k; destruct H
+      end.
 
 
   Definition init_ckind : ckind     :=  C.
@@ -98,6 +105,7 @@ Module no_es_cl_ECCa <: RED_LANG.
       end.
   Coercion valCa_to_term0 : valCa >-> term0.
 
+
   Definition value_to_term {k} : value k -> term :=
       match k as k return value k -> term with
       | C    => fun v => valueC_to_term0 v
@@ -111,7 +119,7 @@ Module no_es_cl_ECCa <: RED_LANG.
   Coercion value_to_term : value >-> term.
 
 
-  Definition not_closure (t : term) := match t with Cl_t _ => False | _ => True end.
+  (*Definition not_closure (t : term) := match t with Cl_t _ => False | _ => True end.*)
 
   Inductive red : ckind -> Type :=
   | rAppLam    : forall k, CECa k -> term         -> term         -> red k
@@ -172,6 +180,14 @@ Module no_es_cl_ECCa <: RED_LANG.
     destruct k;
     inversion H;
     reflexivity.
+  Qed.
+
+
+  Lemma proper_death : forall k, dead_ckind k -> ~ exists (r : redex k), True.
+  Proof.
+    intros k H [r _].
+    destruct r; destruct_all_CECa; 
+    solve [inversion H].
   Qed.
 
 
@@ -318,191 +334,210 @@ destruct t1, t2; destruct n0, n; autof ].
       end.
 
 
-  Inductive decomp (k : ckind) : Set :=
-  | d_red : forall k', redex k' -> context k k' -> decomp k
-  | d_val : value k -> decomp k.
-  Arguments d_val {k} _. Arguments d_red {k} {k'} _ _.
-
-
-  Definition decomp_to_term {k} (d : decomp k) : term :=
-      match d with
-      | d_val v      => value_to_term v
-      | d_red _ r c0 => c0[r]
-      end.
-  Coercion decomp_to_term : decomp >-> term.
-
-
-  Definition only_empty t k := 
-      forall t' {k'} (c : context k k'), c[t'] = t -> ~ dead_ckind k' -> 
-          k = k' /\ c ~= [.](k).
-
-  Definition only_trivial t k := 
-      forall t' {k'} (c : context k k'),  c[t'] = t -> ~ dead_ckind k' -> 
-          k = k' /\ c ~= [.](k) \/ exists (v : value k'), t' = v.
-
-(*
   Lemma valCa_is_valECa : 
-      forall v1 : valCa, exists v2 : value ECa, 
-          (valCa_to_term0 v1 : term) = value_to_term v2.
+      forall v1 : valCa, exists v2 : value ECa,  value_to_term v2 = valCa_to_term0 v1.
 
-  Proof with try rewrite <- value_C_to_term_is in *; auto.
+  Proof with auto.
     destruct v1; intros.
-    - exists (vECaVar n)...
-    - exists (vECaApp v1 v); simpl...
-  Qed.*)
+    - exists (vECaCa (vCaVar n))...
+    - exists (vECaCa (vCaApp v1 v))...
+  Qed.
 
 
-  Lemma value_trivial : forall {k} (v : value k), only_trivial v k.
+  Lemma value_trivial1 : forall {k} (v : value k) ec t, 
+                             ~dead_ckind (k+>ec) -> ec:[t] = v ->
+                                 exists (v' : value (k+>ec)), t = v'.
   Proof.
-    intros k1 v t k2 c; revert t.
-    induction c.
-
-    - intuition.
-
-    - intros t H H0.
-      right.
-
-      destruct IHc with (ec0:[t]) as [(H1, H2) | (v0, H1)];
-          try solve [ auto using death_propagation ];
-          dep_subst;
-      [ destruct ec0; destruct v;  dependent destruction H
-      | destruct ec0; destruct v0; dependent destruction H1 ];
-
-      try solve
-      [ simpl; eautof | apply valCa_is_valECa | destruct t0; discriminate ].
-eexists (vECaCa _); simpl; eauto.
-destruct v; inversion x; subst.
-eexists (vECaCa _); simpl; eauto.
-destruct v; inversion x; subst; simpl; eauto.
-eexists (vECaCa _); simpl; eauto.
-destruct v0; inversion x; subst.
-eexists (vECaCa _); simpl; eauto.
-destruct v0; inversion x; subst. simpl; eauto.
+    intros k v ec t H H0.
+    destruct ec, v; 
+        try match goal with H : _ = _ (vECaCa ?v) |- _ => destruct v end;
+        inversion H0; subst; 
+    solve 
+    [ simpl; eautof
+    | eexists (vECaCa _); simpl; eauto ].
   Qed.
 
 
   Lemma value_redex : forall {k} (v : value k) (r : redex k), 
                           value_to_term v <> redex_to_term r.
   Proof.
-    intros k v r.
+    intros k v r H.
 
     dependent destruction r; dependent destruction v; 
-    simpl;
-    try match goal with 
-    | |- App (term0_to_term (valCa_to_term0 ?v)) _ <> _ => dependent_destruction2 v
-    end;
-
-    try solve [ discriminate | tauto ].
-destruct v as [? | v v']; [| dependent_destruction2 v]; discriminate.
-destruct v as [? | v v']; [| dependent_destruction2 v]; discriminate.
-destruct v as [? | v v']; [| dependent_destruction2 v]; discriminate.
-destruct v; discriminate.
-destruct v; discriminate.
+    inversion H;
+    repeat match goal with 
+    | H : _ (valCa_to_term0 ?v) = _ |- _ => destruct v; inversion H
+    end.
   Qed.
 
-
-  Lemma ot_subterm_val : 
-      forall t t0 ec k, only_trivial t k -> ec:[t0] = t -> ~ dead_ckind (k+>ec) ->
-          exists v : value (k+>ec), t0 = v.
-
-  Proof with auto.
-    intros t t0 ec k H H0 H1.
-    destruct (H t0 _ (ec =: [.])) as [(?, H3) | (v, ?)]...
-    - discriminateJM H3.
-    - exists v; destruct k...
-  Qed.
+End Lam_ClES_NO_PreLang.
 
 
-  Lemma plug_compose  : 
-      forall {k1 k2 k3} (c0 : context k1 k2) (c1 : context k3 k1) t, 
-          (c0 ~+ c1)[t] = c1[c0[t]].
+
+
+Module Lam_ClES_NO_Strategy <: STRATEGY_STEP Lam_ClES_NO_PreLang.
+
+  Import Lam_ClES_NO_PreLang.
+
+
+  Inductive interm_dec k : Set :=
+  | in_red  : redex k -> interm_dec k
+  | in_term : term -> elem_context -> interm_dec k
+  | in_val  : value k -> interm_dec k
+  | in_dead : interm_dec k.
+  Arguments in_red {k} _.    Arguments in_val {k} _.
+  Arguments in_term {k} _ _. Arguments in_dead {k}.
+
+
+  Definition dec_term t k : interm_dec k :=
+
+      match k as k0 return interm_dec k0 with 
+      | C    => match t with
+                | App t1 t2   => in_term t1 (ap_r t2)
+                | Var i       => in_val (vCVar i)
+                | Lam t1      => in_term t1 lam_c
+                | Cl_t (Cl (Var0 i) e)     => in_red (rSubVar C I i e)
+                | Cl_t (Cl (Lam0 t) e)     => in_red (rSubLam t e)
+                | Cl_t (Cl (App0 t1 t2) e) => in_red (rSubApp C I t1 t2 e)
+                | OpVar i e g => in_red (rSubOpVar C I i e g)
+                end
+      | ECa  => match t with
+                | App t1 t2 => in_term t1 (ap_r t2)
+                | Var i     => in_val (vECaCa (vCaVar i))
+                | Lam t1    => in_val (vECaLam t1)
+                | Cl_t (Cl (Var0 i) e)     => in_red (rSubVar ECa I i e)
+                | Cl_t (Cl (Lam0 t) e)     => in_val (vECaLam_cl t e)
+                | Cl_t (Cl (App0 t1 t2) e) => in_red (rSubApp ECa I t1 t2 e)
+                | OpVar i e g   => in_red (rSubOpVar ECa I i e g)
+                end
+      | CBot => in_dead
+      end.
+
+
+  Definition dec_context ec k : value (k+>ec) -> interm_dec k :=
+
+      match ec as ec, k as k return value (k+>ec) -> interm_dec k with
+
+      | lam_c, C      => fun v => in_val (vCLam v)
+      | lam_c, ECa    => fun _ => in_dead
+      | lam_c, CBot   => fun _ => in_dead
+
+      | ap_r t, C     => fun v => 
+                             match v with
+                             | vECaLam t0      => in_red (rAppLam C I t0 t)
+                             | vECaLam_cl t0 e => in_red (rAppLam_cl C I t0 e t)
+                             | vECaCa v        => in_term t (ap_l v)
+                             | _ => @in_dead C
+                             end
+      | ap_r t, ECa   => fun v => 
+                             match v with
+                             | vECaLam t0      => in_red (rAppLam ECa I t0 t)
+                             | vECaLam_cl t0 e => in_red (rAppLam_cl ECa I t0 e t)
+                             | vECaCa v        => in_term t (ap_l v)
+                             | _ => @in_dead ECa
+                             end
+      | ap_r t, CBot  => fun _ => in_dead
+       
+
+      | ap_l v0, C    => fun v => in_val (vCApp v0 v)
+      | ap_l v0, ECa  => fun v => in_val (vECaCa (vCaApp v0 v))
+      | ap_l v0, CBot => fun _ => in_dead
+
+      end.
+
+
+  Lemma dec_term_correct : 
+      forall (t : term) k, match dec_term t k with
+      | in_red r      => t = r
+      | in_val v      => t = v
+      | in_term t' ec => t = ec:[t']
+      | in_dead       => dead_ckind k 
+      end.
+
   Proof.
-    induction c0; intros.
-    - auto.
-    - apply IHc0.
+    destruct k, t; 
+    try match goal with c : closure |- _ => 
+        destruct c as [t0]; destruct t0 
+    end; 
+    solve [ simpl; auto ].
   Qed.
 
 
-  Lemma ot_propagation : 
-      forall t ec k, only_trivial ec:[t] k -> only_trivial t (k+>ec).
-
-  Proof with eauto.
-    intros t ec k H.
-    intros t' k' c H1 H2.
-    destruct (H t' _ (c ~+ ec =: [.])) as [(?, H3) | ?]... 
-    - rewrite plug_compose; subst...
-    - destruct c; discriminateJM H3.
+  Lemma dec_term_from_dead : forall t k, dead_ckind k -> dec_term t k = in_dead.
+  Proof.
+    intros t k H.
+    destruct k;
+    solve [ autof ].
   Qed.
 
 
-  Lemma trivial_val_red : 
-      forall k t, ~dead_ckind k -> only_trivial t k ->
-          (exists (v : value k), t = v) \/ (exists (r : redex k), t = r).
+  Lemma dec_term_next_alive : 
+      forall t k t0 ec0, dec_term t k = in_term t0 ec0 -> ~ dead_ckind (k+>ec0).
 
-  Proof with simpl; eautof.
-    intros k t; revert k.
-    induction t;
-        intros k G H;
-        destruct k.
+  Proof.
+    intros t k t0 ec0 H.
 
-    - left; eexists (vCVar _)...
+    destruct t, k;
+    try match goal with c : closure |- _ => 
+        destruct c as [tt0]; destruct tt0 
+    end;
+        inversion H; subst; 
 
-    - left; eexists (vECaCa (vCaVar _))...
-
-    - autof.
-
-    - destruct (ot_subterm_val _ t lam_c _ H)...
-      subst.
-      left; eexists (vCLam _)...
-
-    - left; eexists (vECaLam _)...
-
-    - autof.
-
-    - destruct (ot_subterm_val _ t1 (ap_r t2) _ H) as (v, H0)...
-      subst.
-      simpl in v; dependent destruction v.
-      + right; eexists (rAppLam C I _ _)...
-      + right; eexists (rAppLam_cl C I _ _ _)...
-      + destruct (ot_subterm_val _ t2 (ap_l v) _ H) as (v0, H0)...
-        subst.
-        left; eexists (vCApp _ _)...
-
-      (* almost "copy-past" of the previous case *)
-    - destruct (ot_subterm_val _ t1 (ap_r t2) _ H) as (v, H0)...
-      subst.
-      simpl in v; dependent destruction v.
-      + right; eexists (rAppLam ECa I _ _)...
-      + right; eexists (rAppLam_cl ECa I _ _ _)...
-      + destruct (ot_subterm_val _ t2 (ap_l v) _ H) as (v0, H0)...
-        subst.
-        left; eexists (vECaCa (vCaApp _ _))...
-
-    - autof.
-
-    - right.
-      destruct c as [[i | t | t1 t2] e].
-      + eexists (rSubVar C I _ _)...
-      + eexists (rSubLam _ _)...
-      + eexists (rSubApp C I _ _ _)...
-
-    - destruct c as [[i | t | t1 t2] e].
-      + right; eexists (rSubVar ECa I _ _)...
-      + left; eexists (vECaLam_cl _ _)...
-      + right; eexists (rSubApp ECa I _ _ _)... 
-
-    - autof.
-
-    - right.
-      eexists (rSubOpVar C I _ _ _)...
-
-    - right.
-      eexists (rSubOpVar ECa I _ _ _)...
-
-    - autof.
+    solve [ auto ].
   Qed.
 
 
+  Lemma dec_context_correct : 
+      forall ec k v, match dec_context ec k v with
+      | in_red r      => ec:[v] = r
+      | in_val v'     => ec:[v] = v'
+      | in_term t ec' => ec:[v] = ec':[t]
+      | in_dead       => dead_ckind (k+>ec)
+      end.
+
+  Proof.
+    intros ec k v.
+    destruct k, ec; dependent destruction v;
+    simpl;
+    solve [ auto ].
+  Qed.
+
+
+  Lemma dec_context_from_dead : forall ec k v, 
+      dead_ckind (k+>ec) -> dec_context ec k v = in_dead.
+
+  Proof.
+    intros ec k v H.
+    destruct ec, k;
+    solve [ autof ].
+  Qed.
+
+
+  Lemma dec_context_next_alive : forall ec k v {t ec0}, 
+      dec_context ec k v = in_term t ec0 -> ~ dead_ckind (k+>ec0).
+
+  Proof.
+    intros ec k v t ec0 H.
+    destruct ec, ec0, k; dependent destruction v;  
+    solve [ autof ].
+  Qed.
+
+End Lam_ClES_NO_Strategy.
+
+
+
+
+Module Lam_ClES_NO_Ref_minus <: RED_REF_LANG_minus.
+
+  Module SX := Lam_ClES_NO_PreLang.
+  Module ST := Lam_ClES_NO_Strategy.
+  Module RED_Props := Lam_ClES_NO_PreLang.
+
+  Export Lam_ClES_NO_PreLang Lam_ClES_NO_Strategy.
+
+
+  
+(*
   Lemma dead_context_dead : 
       forall {k1 k2}, context k1 k2 -> dead_ckind k1 -> dead_ckind k2.
 
@@ -511,419 +546,34 @@ destruct v; discriminate.
     induction 1.
     - trivial.
     - apply death_propagation...
-  Qed.
+  Qed.*)
 
 
-  Lemma proper_death : forall k, dead_ckind k -> 
-                           ~ exists k' (c : context k k') (r : redex k'), True.
-  Proof with eauto.
-    intros k H H0.
-    destruct k;
 
-    (*1*)try solve [discriminate H].
-
-    (*2*)destruct H0 as (k', (c, (r, _))).
-         assert (dead_ckind k').
-         + eapply dead_context_dead...
-         + dependent destruction r;
-           try match goal with
-           | H : CECa ?k |- _ => try destruct k; destruct H
-           end;
-           solve [discriminate H0].
-  Qed.
-
-
-(*
-  (* Contexts from the Johan Munk's paper *)
-  (* To refactor *)
-  Inductive ckind_IO := Aio | Cio | Dio.
-
-  Inductive context_IO : ckind_IO -> Set :=
-  | hole_io   : context_IO Aio
-  | ap_l_io   : context_IO Cio -> valCa -> context_IO Aio
-  | lam_c_io  : context_IO Aio -> context_IO Aio
-
-  | a_is_c_io : context_IO Aio -> context_IO Cio
-  | ap_r_io   : context_IO Cio -> term -> context_IO Cio
-
-  | c_is_d_io : context_IO Cio -> context_IO Dio
-  | stag_c_io : context_IO Dio -> sub_tag -> context_IO Dio.
-
-  Definition a_is_d_io c := c_is_d_io (a_is_c_io c).
-
-
-  Definition context_to_IO {k1 k2} (c : context k1 k2) : 
-               match k2 with  
-               | C => context_IO Aio | ECa => context_IO Cio 
-               | D => context_IO Dio | CBot => unit
-               end.
-  dependent induction c.
-
-  destruct k1.
-  exact hole_io.
-  exact (a_is_c_io hole_io).
-  exact (a_is_d_io hole_io).
-  exact ().
-
-  remember ec0.
-  destruct k2, e; simpl.
-  exact (lam_c_io IHc).
-  exact (ap_r_io (a_is_c_io IHc) t).
-  exact (ap_l_io (a_is_c_io IHc) v).
-  exact (stag_c_io (a_is_d_io IHc) s).
-  exact ().
-  exact (ap_r_io IHc t).
-  exact (ap_l_io IHc v).
-  exact (stag_c_io (c_is_d_io IHc) s).
-  exact ().
-  exact ().
-  exact ().
-  exact (stag_c_io IHc s).
-  exact ().
-  exact ().
-  exact ().
-  exact ().
-  Defined.
-
-
-
-  Definition context_from_IO {k} (c : context_IO k) : 
-               match k with  
-               | Aio => context C C | Cio => context C C + context C ECa 
-               | Dio => context C C + context C ECa + context C D
-               end.
-
-  dependent induction c.
-
-  exact [.].
-
-  destruct IHc;
-  exact (ap_l v=:c0).
-
-  exact (lam_c=:IHc).
-
-  exact (inl IHc).
-
-  destruct IHc;
-  exact (inr (ap_r t=:c0)).
-
-  exact (inl IHc).
-
-  destruct IHc as [[c0 | c0] | c0];
-  exact (inr (stag_c s=:c0)).
-  Defined.
-
-
-
-  Lemma to_from_IO_is_id : 
-            forall k (c : context_IO k),
-                match k as k return context_IO k -> Prop with
-                | Cio => fun c =>
-                    c = match context_from_IO c with 
-                    | inl c => a_is_c_io (context_to_IO c) 
-                    | inr c => context_to_IO c 
-                    end
-                | Aio => fun c => c = context_to_IO (context_from_IO c)
-                | Dio => fun c =>
-                    c = match context_from_IO c with 
-                    | inl (inl c) => a_is_d_io (context_to_IO c) 
-                    | inl (inr c) => c_is_d_io (context_to_IO c) 
-                    | inr c => context_to_IO c 
-                    end
-                end c.
-  Proof.
-    induction c; simpl;
-    auto;
-    try (destruct (context_from_IO c));
-    try destruct s0;
-    simpl; try unfold a_is_d_io in *; try congruence.
-  Qed.
-
-
-  Lemma from_to_IO_is_id : 
-            forall k (c : context C k),
-                match k as k return context C k -> Prop with
-                | C => fun c => c = context_from_IO (context_to_IO c)
-                | ECa => fun c => inr c = context_from_IO (context_to_IO c)
-                | D => fun c => inr c = context_from_IO (context_to_IO c)
-                | CBot => fun c => True
-                end c.
-  Proof.
-    induction c. 
-    simpl; auto.
-    
-    destruct k2, ec0; simpl; try rewrite <- IHc; try congruence; auto.
-  Qed.
-
-
-  Fixpoint plug_IO t {k} (c : context_IO k) :=
-      match c with
-      | hole_io       => t
-      | ap_l_io c' v  => plug_IO (App (v : term) t) c'
-      | lam_c_io c'   => plug_IO (Lam t) c'
-      | a_is_c_io c'  => plug_IO t c'
-      | ap_r_io c' t' => plug_IO (App t t') c'
-      | c_is_d_io c'  => plug_IO t c'
-      | stag_c_io c' (n, st_sub t')  => plug_IO (Sub t n t') c'
-      | stag_c_io c' (n, st_shift m) => plug_IO (Shift t n m) c'
-      end.
-
-
-  Lemma plug_compatible : 
-          forall {k1 k2} (c : context k1 k2) t,
-              match k2 as k2 return context k1 k2 -> Prop with
-              | CBot => fun _ => True
-              | k2   => fun c => c[t] = plug_IO t (context_to_IO c) 
-              end c.
-  Proof.
-    induction c.
-    destruct k1; auto.
-
-    destruct k2, ec0; destruct_all sub_tag; destruct_all substitut; simpl in *; auto.
-  Qed.
-
-
-  Lemma plug_compatible2 : 
-          forall {k} (c : context_IO k) (t : term),
-              plug_IO t c =
-              match k as k return context_IO k -> term with
-              | Aio => fun c => (context_from_IO c)[t]
-              | Cio => fun c => match context_from_IO c with 
-                                | inl c | inr c => c[t] end
-              | Dio => fun c => match context_from_IO c with 
-                                | inl (inl c) | inl (inr c) | inr c => c[t] end
-              end c.
-  Proof.
-    intros.
-    symmetry.
-    destruct k.
-    rewrite (to_from_IO_is_id Aio) at 2.
-    apply @plug_compatible with (k2 := C).
-
-    rewrite (to_from_IO_is_id Cio) at 2.
-    destruct (context_from_IO c).
-    simpl.
-    apply @plug_compatible with (k2 := C).
-    apply @plug_compatible with (k2 := ECa).
-
-    rewrite (to_from_IO_is_id Dio) at 2.
-    destruct (context_from_IO c) as [[c0 | c0] | c0];
-    simpl.
-    apply @plug_compatible with (k2 := C).
-    apply @plug_compatible with (k2 := ECa).
-    apply @plug_compatible with (k2 := D).
-  Qed.
-  *)
-
-End no_es_cl_ECCa.
-
-
-
-
-Module no_es_cl_ECCa_Ref <: RED_REF_LANG.
-
-  Module R  := no_es_cl_ECCa.
-  Module RF := RED_LANG_Facts R.
-  Export R.
-  Import RF.
-
-
-  Module DEC <: REF_STEP R.
-
-    Inductive interm_dec k : Set :=
-    | in_red  : redex k -> interm_dec k
-    | in_term : term -> elem_context -> interm_dec k
-    | in_val  : value k -> interm_dec k
-    | in_dead : interm_dec k.
-    Arguments in_red {k} _.    Arguments in_val {k} _.
-    Arguments in_term {k} _ _. Arguments in_dead {k}.
-
-
-    Definition dec_term t k : interm_dec k :=
-
-        match k as k0 return interm_dec k0 with 
-        | C    => match t with
-                  | App t1 t2   => in_term t1 (ap_r t2)
-                  | Var i       => in_val (vCVar i)
-                  | Lam t1      => in_term t1 lam_c
-                  | Cl_t (Cl (Var0 i) e)     => in_red (rSubVar C I i e)
-                  | Cl_t (Cl (Lam0 t) e)     => in_red (rSubLam t e)
-                  | Cl_t (Cl (App0 t1 t2) e) => in_red (rSubApp C I t1 t2 e)
-                  | OpVar i e g => in_red (rSubOpVar C I i e g)
-                  end
-        | ECa  => match t with
-                  | App t1 t2 => in_term t1 (ap_r t2)
-                  | Var i     => in_val (vECaCa (vCaVar i))
-                  | Lam t1    => in_val (vECaLam t1)
-                  | Cl_t (Cl (Var0 i) e)     => in_red (rSubVar ECa I i e)
-                  | Cl_t (Cl (Lam0 t) e)     => in_val (vECaLam_cl t e)
-                  | Cl_t (Cl (App0 t1 t2) e) => in_red (rSubApp ECa I t1 t2 e)
-                  | OpVar i e g   => in_red (rSubOpVar ECa I i e g)
-                  end
-        | CBot => in_dead
-        end.
-
-
-    Definition dec_context ec k : value (k+>ec) -> interm_dec k :=
-
-        match ec as ec, k as k return value (k+>ec) -> interm_dec k with
-
-        | lam_c, C      => fun v => in_val (vCLam v)
-        | lam_c, ECa    => fun _ => in_dead
-        | lam_c, CBot   => fun _ => in_dead
-
-        | ap_r t, C     => fun v => 
-                               match v with
-                               | vECaLam t0      => in_red (rAppLam C I t0 t)
-                               | vECaLam_cl t0 e => in_red (rAppLam_cl C I t0 e t)
-                               | vECaCa v        => in_term t (ap_l v)
-                               | _ => @in_dead C
-                               end
-        | ap_r t, ECa   => fun v => 
-                               match v with
-                               | vECaLam t0      => in_red (rAppLam ECa I t0 t)
-                               | vECaLam_cl t0 e => in_red (rAppLam_cl ECa I t0 e t)
-                               | vECaCa v        => in_term t (ap_l v)
-                               | _ => @in_dead ECa
-                               end
-        | ap_r t, CBot  => fun _ => in_dead
-       
-
-        | ap_l v0, C    => fun v => in_val (vCApp v0 v)
-        | ap_l v0, ECa  => fun v => in_val (vECaCa (vCaApp v0 v))
-        | ap_l v0, CBot => fun _ => in_dead
-
-        end.
-
-
-    Lemma dec_term_correct : 
-        forall (t : term) k, match dec_term t k with
-        | in_red r      => t = r
-        | in_val v      => t = v
-        | in_term t' ec => t = ec:[t']
-        | in_dead       => dead_ckind k 
-        end.
-
-    Proof.
-      destruct k, t; 
-      try match goal with c : closure |- _ => 
-          destruct c as [t0]; destruct t0 
-      end; 
-      solve [ simpl; auto ].
-    Qed.
-
-
-    Lemma dec_term_from_dead : forall t k, dead_ckind k -> dec_term t k = in_dead.
-    Proof.
-      intros t k H.
-      destruct k;
-      solve [ autof ].
-    Qed.
-
-
-    Lemma dec_term_next_alive : 
-        forall t k t0 ec0, dec_term t k = in_term t0 ec0 -> ~ dead_ckind (k+>ec0).
-
-    Proof.
-      intros t k t0 ec0 H.
-
-      destruct t, k;
-      try match goal with c : closure |- _ => 
-          destruct c as [tt0]; destruct tt0 
-      end;
-          inversion H; subst; 
-
-      solve [ auto ].
-    Qed.
-
-
-    Lemma dec_context_correct : 
-        forall ec k v, match dec_context ec k v with
-        | in_red r      => ec:[v] = r
-        | in_val v'     => ec:[v] = v'
-        | in_term t ec' => ec:[v] = ec':[t]
-        | in_dead       => dead_ckind (k+>ec)
-        end.
-
-    Proof.
-      intros ec k v.
-      destruct k, ec; dependent destruction v;
-      simpl;
-      solve [ auto ].
-    Qed.
-
-
-    Lemma dec_context_from_dead : forall ec k v, 
-        dead_ckind (k+>ec) -> dec_context ec k v = in_dead.
-
-    Proof.
-      intros ec k v H.
-      destruct ec, k;
-      solve [ autof ].
-    Qed.
-
-
-    Lemma dec_context_next_alive : forall ec k v {t ec0}, 
-        dec_context ec k v = in_term t ec0 -> ~ dead_ckind (k+>ec0).
-
-    Proof.
-      intros ec k v t ec0 H.
-      destruct ec, ec0, k; dependent destruction v;  
-      solve [ autof ].
-    Qed.
-
-  End DEC.
-
-  Export DEC.
-
-
-  Lemma redex_trivial : forall {k} (r : redex k), only_trivial r k.
+  Lemma redex_trivial1 : forall {k} (r : redex k) ec t,
+                             ~dead_ckind (k+>ec) -> ec:[t] = r -> 
+                                 exists (v : value (k+>ec)), t = v.
   Proof with auto.
-    intros k1 r t k2 c; revert t.
-    induction c.
-    - intuition.
-    - intros.
-      right.
-
-      destruct IHc with (ec0:[t]) as [(H1, H2) | (v0, H1)];
-          try solve [auto using death_propagation];
-          dep_subst; simpl in *;
-      match goal with
-      | Hvr : ec0 :[ t ] = _ ?vr |- _ => 
-            destruct ec0; destruct vr; 
-            simpl in Hvr;
-            try match type of Hvr with _ = _ (valCa_to_term0 ?v) => destruct v end;
-            dependent_destruction2 Hvr
-      end;
-      try match goal with
-      | H : CECa ?k |- _ => try destruct k; destruct H
-      end;
-
-      try solve 
-      [ simpl; eautof 
-      | apply valCa_is_valECa
-      | eexists (vECaLam _); simpl; auto 
-      | eexists (vECaLam_cl _ _); simpl; auto 
-      | eexists (vECaCa _); simpl; auto 
-      | dependent destruction v; discriminate ].
+    intros k r ec t H H0.
+    destruct ec, r; destruct_all_CECa; inversion H0; subst;
+    solve 
+    [ eexists (vECaLam _); reflexivity
+    | eexists (vECaLam_cl _ _); reflexivity 
+    | match goal with H: _ (valCa_to_term0 ?v) = ?r |- _ => 
+          destruct v; inversion H 
+      end].
   Qed.
 
 
-  Inductive subterm_one_step : term -> term -> Prop :=
-  | st_1 : forall t t0 ec, t = ec:[t0] -> subterm_one_step t0 t.
 
+  Definition subterm_one_step t0 t := exists ec, t = ec:[t0].
 
   Lemma wf_st1 : well_founded subterm_one_step.
-  Proof.
-    RED_REF_LANG_Help.prove_st_wf;
-
-    inversion H1; dep_subst; 
-    auto.
-  Qed.
+  Proof. RED_REF_LANG_Help.prove_st_wf. Qed.
 
 
   Definition subterm_order := clos_trans_1n term subterm_one_step.
-  Notation " a <| b " := (subterm_order a b) (at level 40, no associativity).
+  Notation "t1 <| t2" := (subterm_order t1 t2) (at level 40, no associativity).
   Definition wf_sto : well_founded subterm_order := wf_clos_trans_l _ _ wf_st1.
 
 
@@ -935,13 +585,12 @@ Module no_es_cl_ECCa_Ref <: RED_REF_LANG.
                 | _, _           => False
                 end
       end.
-  Notation "k , t |~  ec1 << ec2 " := (ec_order k t ec1 ec2) (at level 40, no associativity).
+  Notation "k , t |~  ec1 << ec2 " := (ec_order k t ec1 ec2) 
+               (at level 40, no associativity).
 
 
   Lemma wf_eco : forall k t, well_founded (ec_order k t).
-  Proof.
-    RED_REF_LANG_Help.prove_ec_wf.
-  Qed.
+  Proof. RED_REF_LANG_Help.prove_ec_wf. Qed.
 
 
   Lemma ec_order_antisym : forall k t ec ec0, 
@@ -996,6 +645,28 @@ Module no_es_cl_ECCa_Ref <: RED_REF_LANG.
     destruct k, ec0, ec1;
     inversion H;
     solve [auto].
+  Qed.
+
+
+
+
+  Definition only_empty t k := 
+      forall t' {k'} (c : context k k'), c[t'] = t -> ~ dead_ckind k' -> 
+          k = k' /\ c ~= [.](k).
+
+  Definition only_trivial t k := 
+      forall t' {k'} (c : context k k'),  c[t'] = t -> ~ dead_ckind k' -> 
+          k = k' /\ c ~= [.](k) \/ exists (v : value k'), t' = v.
+
+
+  Lemma death_propagation2 : 
+      forall k ec, ~ dead_ckind (k+>ec) -> ~ dead_ckind k.
+
+  Proof.
+    intuition.
+    apply H.
+    apply death_propagation.
+    assumption.
   Qed.
 
 
@@ -1121,30 +792,28 @@ Module no_es_cl_ECCa_Ref <: RED_REF_LANG.
       trivial ].
   Qed.
 
-End no_es_cl_ECCa_Ref.
+End Lam_ClES_NO_Ref_minus.
 
+
+
+Module Lam_ClES_NO_Ref := mk_RedRefLang Lam_ClES_NO_Ref_minus.
 
 
 
 Require Import refocusing_semantics_derivation.
 Require Import refocusing_machine.
 
-Module no_es_cl_ECCa_REF_SEM := RedRefSem no_es_cl_ECCa_Ref.
-Module ECCa_es_cl_EAM        := ProperEAMachine no_es_cl_ECCa no_es_cl_ECCa_REF_SEM.
+Module Lam_ClES_NO_RefSem := RedRefSem Lam_ClES_NO_Ref.
+Module Lam_ClES_NO_EAM    := ProperEAMachine Lam_ClES_NO_Ref.R Lam_ClES_NO_RefSem.
 
 
 
-Module ECCa_es_cl_EAM_safe <: AM_SAFE_REGION ECCa_es_cl_EAM.
+Module Lam_ClES_NO_EAM_safe <: AM_SAFE_REGION Lam_ClES_NO_EAM.
 
-  Import ECCa_es_cl_EAM.
-  Import no_es_cl_ECCa.
+  Import Lam_ClES_NO_EAM.
+  Import Lam_ClES_NO_PreLang.
 
 
-  (*Fixpoint ec_in_context ec {k1 k2} (c : context k1 k2) :=
-    match c with
-    | [.]       => False
-    | ec' =: c' => ec' = ec \/ ec_in_context ec c'
-    end.*)
 
   Fixpoint good_context {k1 k2} (c : context k1 k2) :=
       match c with
@@ -1258,7 +927,9 @@ Module ECCa_es_cl_EAM_safe <: AM_SAFE_REGION ECCa_es_cl_EAM.
     intros.
     destruct st.
     - right. 
-      destruct t as [? | ? | tt1 tt2 | [[? | ? | ? ?] [ | (?, ?) ?]] | ? [ | (?, ?) ?] ?], k2;
+      destruct t as 
+          [? | ? | tt1 tt2 | [[? | ? | ? ?] [ | (?, ?) ?]] | ? [ | (?, ?) ?] ?], 
+          k2;
       try destruct tt1, tt2;
 
       destruct H as [? [? ?]];
@@ -1281,15 +952,15 @@ Module ECCa_es_cl_EAM_safe <: AM_SAFE_REGION ECCa_es_cl_EAM.
                            | apply t_cterm; simpl; auto].
   Qed.
 
-End ECCa_es_cl_EAM_safe.
+End Lam_ClES_NO_EAM_safe.
 
 
 
 
-Module ECCa_es_cl_EAM_minus <: DET_ABSTRACT_MACHINE.
+Module Lam_ClES_NO_EAM_minus <: DET_ABSTRACT_MACHINE.
 
-  Module AM := ECCa_es_cl_EAM.
-  Import no_es_cl_ECCa.
+  Module AM := Lam_ClES_NO_EAM.
+  Import Lam_ClES_NO_PreLang.
 
   Definition term := term0.
   Definition value := AM.value.
@@ -1314,32 +985,32 @@ Module ECCa_es_cl_EAM_minus <: DET_ABSTRACT_MACHINE.
   Inductive eval : term -> value -> Prop :=
   | e_intro : forall t v, trans_close (c_init t) (c_final v) -> eval t v.
 
-  Definition next_conf := AM.next_conf.
+  Definition next_conf    := AM.next_conf.
   Definition next_correct := AM.next_correct.
 
-End ECCa_es_cl_EAM_minus.
+End Lam_ClES_NO_EAM_minus.
 
 
 
 
 Require Import abstract_machine_facts.
 
-Module ECCa_es_cl_EAM_minus_InitSafe <: 
-           AM_INIT_SAFE  ECCa_es_cl_EAM_minus  ECCa_es_cl_EAM_safe.
+Module Lam_ClES_NO_EAM_minus_InitSafe <: 
+           AM_INIT_SAFE  Lam_ClES_NO_EAM_minus  Lam_ClES_NO_EAM_safe.
 
-  Import ECCa_es_cl_EAM_minus ECCa_es_cl_EAM_safe.
+  Import Lam_ClES_NO_EAM_minus Lam_ClES_NO_EAM_safe.
 
   Lemma init_safe : forall t, safe (c_init t).
   Proof. simpl; auto. Qed.
 
-End ECCa_es_cl_EAM_minus_InitSafe.
+End Lam_ClES_NO_EAM_minus_InitSafe.
 
 
 
 
-Module ECCa_es_cl_EAM_minus_Progress <: AM_PROGRESS ECCa_es_cl_EAM_minus :=
+Module Lam_ClES_NO_EAM_minus_Progress <: AM_PROGRESS Lam_ClES_NO_EAM_minus :=
 
-    AM_ProgressFromSafety  ECCa_es_cl_EAM_minus  ECCa_es_cl_EAM_safe
-                           ECCa_es_cl_EAM_minus_InitSafe.
+    AM_ProgressFromSafety  Lam_ClES_NO_EAM_minus  Lam_ClES_NO_EAM_safe
+                           Lam_ClES_NO_EAM_minus_InitSafe.
 
 
