lam_no.v
@@ -5,7 +5,8 @@ Require Import reduction_semantics_facts.
 
 
 
-Module no_ECCa <: RED_LANG.
+
+Module Lam_NO_PreLang <: RED_SYNTAX.
 
   Parameter var : Set.
 
@@ -39,7 +40,8 @@ Module no_ECCa <: RED_LANG.
 
   | vCaVar : var -> valCa
   | vCaApp : valCa -> val C -> valCa.
-  
+
+
   Definition value := val.
   Hint Unfold value.
 
@@ -186,7 +188,7 @@ Module no_ECCa <: RED_LANG.
   Proof.
     intros ec t0 t1 H.
     destruct ec;
-    ( injection H; trivial ).
+    solve [ injection H; trivial ].
   Qed.
 
 
@@ -211,27 +213,6 @@ Module no_ECCa <: RED_LANG.
       end.
 
 
-  Inductive decomp (k : ckind) : Set :=
-  | d_red : forall k', redex k' -> context k k' -> decomp k
-  | d_val : value k -> decomp k.
-  Arguments d_val {k} _. Arguments d_red {k} {k'} _ _.
-
-
-  Definition decomp_to_term {k} (d : decomp k) : term :=
-      match d with
-      | d_val v => value_to_term v
-      | d_red _ r c0 => c0[r]
-      end.
-  Coercion decomp_to_term : decomp >-> term.
-
-
-  Definition only_empty t k := 
-      forall t' {k'} (c : context k k'), c[t'] = t -> ~ dead_ckind k' -> 
-          k = k' /\ c ~= [.](k).
-
-  Definition only_trivial t k := 
-      forall t' {k'} (c : context k k'),  c[t'] = t -> ~ dead_ckind k' -> 
-          k = k' /\ c ~= [.](k) \/ exists (v : value k'), t' = v.
 
 
   Lemma valCa_is_valECa : 
@@ -244,24 +225,15 @@ Module no_ECCa <: RED_LANG.
   Qed.
 
 
-  Lemma value_trivial : forall {k} (v : value k), only_trivial v k.
+  Lemma value_trivial1 : forall {k} (v : value k) ec t, 
+                             ~dead_ckind (k+>ec) -> ec:[t] = v ->
+                                 exists (v' : value (k+>ec)), t = v'.
   Proof.
-    intros k1 v t k2 c; revert t.
-    induction c.
-
-    - intuition.
-
-    - intros t H H0.
-      right.
-
-      destruct IHc with (ec0:[t]) as [(H1, H2) | (v0, H1)];
-          try solve [ auto using death_propagation ];
-          dep_subst;
-      [ destruct ec0; destruct v;  dependent destruction H
-      | destruct ec0; destruct v0; dependent destruction H1 ];
-
-      solve
-      [ eautof | apply valCa_is_valECa ].
+    intros k v ec t H H0.
+    destruct ec, v; inversion H0; subst; 
+    solve 
+    [ eautof
+    | auto using valCa_is_valECa ].
   Qed.
 
 
@@ -280,303 +252,193 @@ Module no_ECCa <: RED_LANG.
   Qed.
 
 
-  Lemma ot_subterm_val : 
-      forall t t0 ec k, only_trivial t k -> ec:[t0] = t -> ~ dead_ckind (k+>ec) ->
-          exists v : value (k+>ec), t0 = v.
-
-  Proof with auto.
-    intros t t0 ec k H H0 H1.
-    destruct (H t0 _ (ec =: [.])) as [(?, H3) | (v, ?)]...
-    - discriminateJM H3.
-    - exists v; destruct k...
+  Lemma proper_death : forall k, dead_ckind k -> ~ exists (r : redex k), True.
+  Proof with eauto.
+    intros k H [r _].
+    destruct r; 
+    solve [inversion H].
   Qed.
 
+End Lam_NO_PreLang.
 
-  Lemma plug_compose  : 
-      forall {k1 k2 k3} (c0 : context k1 k2) (c1 : context k3 k1) t, 
-          (c0 ~+ c1)[t] = c1[c0[t]].
+
+
+
+Module Lam_NO_Strategy <: STRATEGY_STEP Lam_NO_PreLang.
+
+  Import Lam_NO_PreLang.
+
+
+  Inductive interm_dec k : Set :=
+  | in_red  : redex k -> interm_dec k
+  | in_term : term -> elem_context -> interm_dec k
+  | in_val  : value k -> interm_dec k
+  | in_dead : interm_dec k.
+  Arguments in_red {k} _.    Arguments in_val {k} _.
+  Arguments in_term {k} _ _. Arguments in_dead {k}.
+
+
+  Definition dec_term t k : interm_dec k :=
+
+      match k as k0 return interm_dec k0 with 
+      | C    => match t with
+                | App t1 t2 => in_term t1 (ap_r t2)
+                | Var x     => in_val (vCVar x)
+                | Lam x t1  => in_term t1 (lam_c x)
+                  end
+      | ECa  => match t with
+                | App t1 t2 => in_term t1 (ap_r t2)
+                | Var x     => in_val (vECaVar x)
+                | Lam x t1  => in_val (vECaLam x t1)
+                end
+      | CBot => in_dead
+      end.
+
+
+  Definition dec_context ec k (v : value (k+>ec)) : interm_dec k :=
+
+      match ec as ec0 return value (k+>ec0) -> interm_dec k with
+
+      | lam_c x  => match k as k0 return value (k0+>lam_c x) -> interm_dec k0 with
+                    | C    => fun v => in_val (vCLam x v)
+                    | ECa  => fun v => in_dead
+                    | CBot => fun v => in_dead
+                    end
+
+      | ap_r t   => match k as k0 return value (k0+>(ap_r t)) -> interm_dec k0 with
+                    | C    => fun v => 
+                                  match v with
+                                  | vECaLam x t0  => in_red (rCApp x t0 t)
+                                  | vECaVar x     => in_term t (ap_l (vCaVar x))
+                                  | vECaApp v1 v2 => in_term t (ap_l (vCaApp v1 v2))
+                                  | _ => @in_dead C
+                                  end
+                    | ECa  => fun v => 
+                                  match v with
+                                  | vECaLam x t0  => in_red (rECaApp x t0 t)
+                                  | vECaVar x     => in_term t (ap_l (vCaVar x))
+                                  | vECaApp v1 v2 => in_term t (ap_l (vCaApp v1 v2))
+                                  | _ => @in_dead ECa
+                                  end
+                    | CBot => fun v => in_dead
+                    end
+
+      | ap_l v0  => match k as k0 return value (k0+>(ap_l v0)) -> interm_dec k0 with
+                    | C    => fun v => in_val (vCApp v0 v)
+                    | ECa  => fun v => in_val (vECaApp v0 v)
+                    | CBot => fun v => in_dead
+                    end
+      end v.
+
+
+  Lemma dec_term_correct : 
+      forall (t : term) k, match dec_term t k with
+      | in_red r      => t = r
+      | in_val v      => t = v
+      | in_term t' ec => t = ec:[t']
+      | in_dead       => dead_ckind k 
+      end.
+
   Proof.
-    induction c0; intros.
-    - auto.
-    - apply IHc0.
+    destruct k, t; simpl; 
+    auto.
   Qed.
 
 
-  Lemma ot_propagation : 
-      forall t ec k, only_trivial ec:[t] k -> only_trivial t (k+>ec).
-
-  Proof with eauto.
-    intros t ec k H.
-    intros t' k' c H1 H2.
-    destruct (H t' _ (c ~+ ec =: [.])) as [(?, H3) | ?]... 
-    - rewrite plug_compose; subst...
-    - destruct c; discriminateJM H3.
-  Qed.
-
-
-  Lemma trivial_val_red : 
-      forall k t, only_trivial t k ->
-          (exists (v : value k), t = v) \/ (exists (r : redex k), t = r).
-
-  Proof with (simpl; eautof).
-    intros k t H.
-    induction t;
-        destruct k.
-    
-    - destruct (ot_subterm_val _ t1 (ap_r t2) _ H) as (v, H0)...
-      subst.
-      simpl in v; dependent destruction v.
-      + right; eexists (rCApp _ _ _)...
-      + destruct (ot_subterm_val _ t2 (ap_l (vCaVar v)) _ H) as (v0, H0)...
-        subst.
-        left; eexists (vCApp (vCaVar _) _)...
-      + destruct (ot_subterm_val _ t2 (ap_l (vCaApp v v1)) _ H) as (v0, H0)...
-        subst.
-        left; eexists (vCApp (vCaApp _ _) _)...
-
-      (* almost "copy-past" of the previous case *)
-    - destruct (ot_subterm_val _ t1 (ap_r t2) _ H) as (v, H0)...
-      subst.
-      simpl in v; dependent destruction v.
-      + right; eexists (rECaApp _ _ _)...
-      + destruct (ot_subterm_val _ t2 (ap_l (vCaVar v)) _ H) as (v0, H0)...
-        subst.
-        left; eexists (vECaApp (vCaVar _) _)...
-      + destruct (ot_subterm_val _ t2 (ap_l (vCaApp v v1)) _ H) as (v0, H0)...
-        subst.
-        left; eexists (vECaApp (vCaApp _ _) _)...
-
-    - left; eexists (vCBot (App _ _))...
-
-    - left; eexists (vCVar _)...
-
-    - left; eexists (vECaVar _)...
-
-    - left; eexists (vCBot (Var _))...
-
-    - destruct (ot_subterm_val _ t (lam_c v) _ H)...
-      subst.
-      left; eexists (vCLam _ _); subst...
-
-    - left; eexists (vECaLam _ _)...
-
-    - left; eexists (vCBot (Lam _ _))...
-  Qed.
-
-
-  Lemma dead_context_dead : 
-      forall {k1 k2}, context k1 k2 -> dead_ckind k1 -> dead_ckind k2.
-
-  Proof with auto.
-    intros ? ? c H; revert c.
-    induction 1.
-    - trivial.
-    - apply death_propagation...
-  Qed.
-
-
-  Lemma proper_death : forall k, dead_ckind k -> 
-                           ~ exists k' (c : context k k') (r : redex k'), True.
-  Proof with eauto.
-    intros k H H0.
+  Lemma dec_term_from_dead : forall t k, dead_ckind k -> dec_term t k = in_dead.
+  Proof.
+    intros t k H.
     destruct k;
-
-    (*1*)try solve [discriminate H].
-
-    (*2*)destruct H0 as (k', (c, (r, _))).
-         assert (dead_ckind k').
-         + eapply dead_context_dead...
-         + dependent destruction r; 
-           discriminate H0.
+    solve [ autof ].
   Qed.
 
-End no_ECCa.
+
+  Lemma dec_term_next_alive : 
+      forall t k t0 ec0, dec_term t k = in_term t0 ec0 -> ~ dead_ckind (k+>ec0).
+
+  Proof.
+    intros t k t0 ec0 H.
+    destruct t, k;
+    solve [ inversion H; subst; 
+            auto ].
+  Qed.
+
+
+  Lemma dec_context_correct : 
+      forall ec k v, match dec_context ec k v with
+      | in_red r      => ec:[v] = r
+      | in_val v'     => ec:[v] = v'
+      | in_term t ec' => ec:[v] = ec':[t]
+      | in_dead       => dead_ckind (k+>ec)
+      end.
+
+  Proof.
+    intros ec k v.
+    destruct k, ec; dependent destruction v;
+    simpl;
+    solve [ auto ].
+  Qed.
+
+
+  Lemma dec_context_from_dead : forall ec k v, 
+      dead_ckind (k+>ec) -> dec_context ec k v = in_dead.
+
+  Proof.
+    intros ec k v H.
+    destruct ec, k;
+    solve [ autof ].
+  Qed.
+
+
+  Lemma dec_context_next_alive : forall ec k v {t ec0}, 
+      dec_context ec k v = in_term t ec0 -> ~ dead_ckind (k+>ec0).
+
+  Proof.
+    intros ec k v t ec0 H.
+    destruct ec, ec0, k; dependent destruction v;  
+    solve [ autof ].
+  Qed.
+
+End Lam_NO_Strategy.
 
 
 
 
-Module no_ECCa_Ref <: RED_REF_LANG.
+Module Lam_NO_Ref_minus <: RED_REF_LANG_minus.
 
-  Module R  := no_ECCa.
-  Module RF := RED_LANG_Facts R.
-  Export R.
-  Import RF.
-
-
-  Module DEC <: REF_STEP R.
-
-    Inductive interm_dec k : Set :=
-    | in_red  : redex k -> interm_dec k
-    | in_term : term -> elem_context -> interm_dec k
-    | in_val  : value k -> interm_dec k
-    | in_dead : interm_dec k.
-    Arguments in_red {k} _.    Arguments in_val {k} _.
-    Arguments in_term {k} _ _. Arguments in_dead {k}.
-
-
-    Definition dec_term t k : interm_dec k :=
-
-        match k as k0 return interm_dec k0 with 
-        | C    => match t with
-                  | App t1 t2 => in_term t1 (ap_r t2)
-                  | Var x     => in_val (vCVar x)
-                  | Lam x t1  => in_term t1 (lam_c x)
-                  end
-        | ECa  => match t with
-                  | App t1 t2 => in_term t1 (ap_r t2)
-                  | Var x     => in_val (vECaVar x)
-                  | Lam x t1  => in_val (vECaLam x t1)
-                  end
-        | CBot => in_dead
-        end.
-
-
-    Definition dec_context ec k (v : value (k+>ec)) : interm_dec k :=
-
-        match ec as ec0 return value (k+>ec0) -> interm_dec k with
-
-        | lam_c x  => match k as k0 return value (k0+>lam_c x) -> interm_dec k0 with
-                      | C    => fun v => in_val (vCLam x v)
-                      | ECa  => fun v => in_dead
-                      | CBot => fun v => in_dead
-                      end
-
-        | ap_r t   => match k as k0 return value (k0+>(ap_r t)) -> interm_dec k0 with
-                      | C    => fun v => 
-                                    match v with
-                                    | vECaLam x t0  => in_red (rCApp x t0 t)
-                                    | vECaVar x     => in_term t (ap_l (vCaVar x))
-                                    | vECaApp v1 v2 => in_term t (ap_l (vCaApp v1 v2))
-                                    | _ => @in_dead C
-                                    end
-                      | ECa  => fun v => 
-                                    match v with
-                                    | vECaLam x t0  => in_red (rECaApp x t0 t)
-                                    | vECaVar x     => in_term t (ap_l (vCaVar x))
-                                    | vECaApp v1 v2 => in_term t (ap_l (vCaApp v1 v2))
-                                    | _ => @in_dead ECa
-                                    end
-                      | CBot => fun v => in_dead
-                      end
-
-        | ap_l v0  => match k as k0 return value (k0+>(ap_l v0)) -> interm_dec k0 with
-                      | C    => fun v => in_val (vCApp v0 v)
-                      | ECa  => fun v => in_val (vECaApp v0 v)
-                      | CBot => fun v => in_dead
-                      end
-        end v.
-
-
-    Lemma dec_term_correct : 
-        forall (t : term) k, match dec_term t k with
-        | in_red r      => t = r
-        | in_val v      => t = v
-        | in_term t' ec => t = ec:[t']
-        | in_dead       => dead_ckind k 
-        end.
-
-    Proof.
-      destruct k, t; simpl; 
-      auto.
-    Qed.
-
-
-    Lemma dec_term_from_dead : forall t k, dead_ckind k -> dec_term t k = in_dead.
-    Proof.
-      intros t k H.
-      destruct k;
-      solve [ autof ].
-    Qed.
-
-
-    Lemma dec_term_next_alive : 
-        forall t k t0 ec0, dec_term t k = in_term t0 ec0 -> ~ dead_ckind (k+>ec0).
-
-    Proof.
-      intros t k t0 ec0 H.
-      destruct t, k;
-      solve [ inversion H; subst; 
-              auto ].
-    Qed.
-
-
-    Lemma dec_context_correct : 
-        forall ec k v, match dec_context ec k v with
-        | in_red r      => ec:[v] = r
-        | in_val v'     => ec:[v] = v'
-        | in_term t ec' => ec:[v] = ec':[t]
-        | in_dead       => dead_ckind (k+>ec)
-        end.
-
-    Proof.
-      intros ec k v.
-      destruct k, ec; dependent destruction v;
-      simpl;
-      solve [ auto ].
-    Qed.
-
-
-    Lemma dec_context_from_dead : forall ec k v, 
-        dead_ckind (k+>ec) -> dec_context ec k v = in_dead.
-
-    Proof.
-      intros ec k v H.
-      destruct ec, k;
-      solve [ autof ].
-    Qed.
-
-
-    Lemma dec_context_next_alive : forall ec k v {t ec0}, 
-        dec_context ec k v = in_term t ec0 -> ~ dead_ckind (k+>ec0).
-
-    Proof.
-      intros ec k v t ec0 H.
-      destruct ec, ec0, k; dependent destruction v;  
-      solve [ autof ].
-    Qed.
-
-  End DEC.
-
-  Export DEC.
+  Module SX := Lam_NO_PreLang.
+  Module ST := Lam_NO_Strategy.
+  Module RED_Props := Lam_NO_PreLang.
+  Module RSF := RED_SYNTAX_Facts SX.
+  Export Lam_NO_PreLang Lam_NO_Strategy.
+  Import RSF.
 
 
 
-  Lemma redex_trivial : forall {k} (r : redex k), only_trivial r k.
+
+  Lemma redex_trivial1 : forall {k} (r : redex k) ec t,
+                             ~dead_ckind (k+>ec) -> ec:[t] = r -> 
+                                 exists (v : value (k+>ec)), t = v.
   Proof with auto.
-    intros k1 r t k2 c; revert t.
-    induction c.
-    - intuition.
-    - intros.
-      right.
-
-      destruct IHc with (ec0:[t]) as [(H1, H2) | (v0, H1)];
-          try solve [auto using death_propagation];
-          dep_subst; simpl in *;
-      match goal with
-      | [Hvr : ec0 :[ t ] = _ ?vr |- _] => 
-            destruct ec0; destruct vr; dependent_destruction2 Hvr
-      end;
-
-      solve 
-      [ eautof 
-      | apply valCa_is_valECa
-      | eexists (vECaLam _ _); simpl; auto 
-      | dependent destruction v; discriminate ].
+    intros k r ec t H H0.
+    destruct ec, r; inversion H0; subst;
+    solve 
+    [ eexists (vECaLam _ _); reflexivity
+    | eauto using valCa_is_valECa
+    | destruct v; inversion H2 ].
   Qed.
 
 
-  Inductive subterm_one_step : term -> term -> Prop :=
-  | st_1 : forall t t0 ec, t = ec:[t0] -> subterm_one_step t0 t.
 
+
+  Definition subterm_one_step t0 t := exists ec, t = ec:[t0].
 
   Lemma wf_st1 : well_founded subterm_one_step.
-  Proof.
-    RED_REF_LANG_Help.prove_st_wf.
-  Qed.
+  Proof. RED_REF_LANG_Help.prove_st_wf. Qed.
 
 
   Definition subterm_order := clos_trans_1n term subterm_one_step.
-  Notation " a <| b " := (subterm_order a b) (at level 40, no associativity).
+  Notation "t1 <| t2" := (subterm_order t1 t2) (at level 40, no associativity).
   Definition wf_sto : well_founded subterm_order := wf_clos_trans_l _ _ wf_st1.
 
 
@@ -588,13 +450,12 @@ Module no_ECCa_Ref <: RED_REF_LANG.
                   | _, _           => False
                   end
       end.
-  Notation "k , t |~  ec1 << ec2 " := (ec_order k t ec1 ec2) (at level 40, no associativity).
+  Notation "k , t |~  ec1 << ec2 " := (ec_order k t ec1 ec2) 
+               (at level 40, no associativity).
 
 
   Lemma wf_eco : forall k t, well_founded (ec_order k t).
-  Proof.
-    RED_REF_LANG_Help.prove_ec_wf.
-  Qed.
+  Proof. RED_REF_LANG_Help.prove_ec_wf. Qed.
 
 
   Lemma ec_order_antisym : forall k t ec ec0, 
@@ -652,15 +513,37 @@ Module no_ECCa_Ref <: RED_REF_LANG.
   Qed.
 
 
+
+
+  Definition only_empty t k := 
+      forall t' {k'} (c : context k k'), c[t'] = t -> ~ dead_ckind k' -> 
+          k = k' /\ c ~= [.](k).
+
+  Definition only_trivial t k := 
+      forall t' {k'} (c : context k k'),  c[t'] = t -> ~ dead_ckind k' -> 
+          k = k' /\ c ~= [.](k) \/ exists (v : value k'), t' = v.
+
+
+  Lemma death_propagation2 : 
+      forall k ec, ~ dead_ckind (k+>ec) -> ~ dead_ckind k.
+
+  Proof.
+    intuition.
+    apply H.
+    apply death_propagation.
+    assumption.
+  Qed.
+
+
   Lemma dec_term_red_empty : 
       forall t k (r : redex k), dec_term t k = in_red r -> only_empty t k.
 
-  Proof with auto.
+  Proof.
     intros t k r H.
     destruct t; 
     inversion H; subst; clear H;
 
-    solve
+    try solve
     [ intros t0 k' c H H0; generalize dependent t0;
 
       induction c;
@@ -772,13 +655,16 @@ Module no_ECCa_Ref <: RED_REF_LANG.
       trivial ].
   Qed.
 
-End no_ECCa_Ref.
+End Lam_NO_Ref_minus.
 
+
+
+Module Lam_NO_Ref := mk_RedRefLang Lam_NO_Ref_minus.
 
 
 
 Require Import refocusing_semantics_derivation.
 Require Import refocusing_machine.
 
-Module no_ECCa_REF_SEM := RedRefSem no_ECCa_Ref.
-Module ECCa_EAM        := ProperEAMachine no_ECCa no_ECCa_REF_SEM.
+Module Lam_NO_RefSem := RedRefSem Lam_NO_Ref.
+Module Lam_NO_EAM    := ProperEAMachine Lam_NO_Ref.R Lam_NO_RefSem.
