miniml.v
@@ -4,7 +4,8 @@ Require Import refocusing_lang.
 Require Import reduction_semantics_facts.
 
 
-Module MiniML_SX <: RED_SYNTAX.
+
+Module MiniML_PreLang <: RED_SYNTAX.
 
   Parameter var : Set.
 
@@ -70,8 +71,9 @@ Module MiniML_SX <: RED_SYNTAX.
   Notation "k +> ec" := (ckind_trans k ec) (at level 50, left associativity).
 
 
+  Definition init_ckind : ckind     := ().
   Definition dead_ckind (_ : ckind) := False.
-  Hint Unfold dead_ckind.
+  Hint Unfold init_ckind dead_ckind.
 
   Inductive context (k1 : ckind) : ckind -> Set :=
   | empty : context k1 k1
@@ -155,7 +157,7 @@ Module MiniML_SX <: RED_SYNTAX.
       | pair_l v       => Pair (v : term) t
       | pair_r t2      => Pair t t2
       end.
-  Notation "ec :[ t ]" := (elem_plug t ec) (at level 0, t at level 99).
+  Notation "ec :[ t ]" := (elem_plug t ec) (at level 0).
 
 
   Lemma elem_plug_injective1 : forall ec {t0 t1}, ec:[t0] = ec:[t1] -> t0 = t1.
@@ -174,40 +176,23 @@ Module MiniML_SX <: RED_SYNTAX.
       | [.]    => t 
       | ec=:c' => plug ec:[t] c'
       end.
-  Notation "c [ t ]" := (plug t c) (at level 0, t at level 99).
+  Notation "c [ t ]" := (plug t c) (at level 0).
 
 
   Definition immediate_ec ec t := exists t', ec:[t'] = t.
-
-End MiniML_SX.
-
-
-
-
-Module MiniML_Ref_minus <: RED_REF_LANG_minus.
-
-  Module SX := MiniML_SX.
-
-  Module RSF := RED_SYNTAX_Facts SX.
-  Export SX.
-  Import RSF.
-
-
-
-  Definition init_ckind : ckind := ().
-  Hint Unfold init_ckind.
 
 
   Lemma death_propagation : 
       forall k, dead_ckind k -> forall ec, dead_ckind (k+>ec).
 
-  Proof.
-    intuition.
-  Qed.
+  Proof. auto. Qed.
+
+
+  Lemma proper_death : forall k, dead_ckind k -> ~ exists (r : redex k), True.
+  Proof. auto. Qed.
 
 
   Parameter subst : var -> term -> term -> term.
-
 
   Definition contract {k} (r : redex k) : option term :=
       match r with
@@ -222,103 +207,160 @@ Module MiniML_Ref_minus <: RED_REF_LANG_minus.
       end.
   Notation contract' := (@contract ()).
 
-(*
-  Inductive decomp (k : ckind) : Set :=
-  | d_red : forall k', redex k' -> context k k' -> decomp k
-  | d_val : value k -> decomp k.
-  Arguments d_val {k} _. Arguments d_red {k} {k'} _ _.
-  Notation decomp' := (decomp ()).
+End MiniML_PreLang.
 
 
-  Definition decomp_to_term {k} (d : decomp k) : term :=
-      match d with
-      | d_val v => value_to_term v
-      | d_red _ r c0 => c0[r]
+
+
+Module MiniML_Strategy <: STRATEGY_STEP MiniML_PreLang.
+
+  Import MiniML_PreLang.
+
+
+  Inductive interm_dec k : Set :=
+  | in_red  : redex k -> interm_dec k
+  | in_term : term -> elem_context -> interm_dec k
+  | in_val  : value k -> interm_dec k
+  | in_dead : interm_dec k.
+  Arguments in_red {k} _.    Arguments in_val {k} _.
+  Arguments in_term {k} _ _. Arguments in_dead {k}.
+
+  Definition dec_term (t : term) k : interm_dec k :=
+      match t with
+      | Z              =>  in_val vZ
+      | S t            =>  in_term t s_c
+      | App t1 t2      =>  in_term t1 (ap_r t2)
+      | Var x          =>  in_val (vVar x)
+      | Lam x t        =>  in_val (vLam x t)
+      | Case t ez x es =>  in_term t (case_c ez x es)
+      | Letv x t e     =>  in_term t (let_c x e)
+      | Fix x t        =>  in_red (rFix x t)
+      | Pair t1 t2     =>  in_term t1 (pair_r t2)
+      | Fst t          =>  in_term t fst_c
+      | Snd t          =>  in_term t snd_c
       end.
-  Coercion decomp_to_term : decomp >-> term.*)
+
+  Definition dec_context (ec : elem_context) k (v : value (k+>ec)) : interm_dec k :=
+      match ec with
+      | s_c             =>  in_val (vS v)
+      | ap_l v0         =>  in_red (rApp v0 v)
+      | ap_r t          =>  in_term t (ap_l v)
+      | case_c ez x es  =>  in_red (rCase v ez x es)
+      | let_c x e       =>  in_red (rLet x v e)
+      | fst_c           =>  in_red (rFst v)
+      | snd_c           =>  in_red (rSnd v)
+      | pair_l v0       =>  in_val (vPair v0 v)
+      | pair_r t        =>  in_term t (pair_l v)
+      end.
 
 
+  Lemma dec_term_correct : 
+      forall (t : term) k, match dec_term t k with
+      | in_red r      => t = r
+      | in_val v      => t = v
+      | in_term t' ec => t = ec:[t']
+      | in_dead       => dead_ckind k 
+      end.
 
-  Lemma value_trivial1 : forall {k} (v : value k) ec t, 
-                             ~dead_ckind (k+>ec) -> ec:[t] = v ->
-                                 exists (v' : value (k+>ec)), t = v'.
+  Proof with auto.
+    destruct k, t; simpl... 
+  Qed.
+
+
+  Lemma dec_term_from_dead : forall t k, dead_ckind k -> dec_term t k = in_dead.
+  Proof.
+    intros ? k H.
+    inversion H.
+  Qed.
+
+
+  Lemma dec_term_next_alive : 
+      forall t k t0 ec0, dec_term t k = in_term t0 ec0 -> ~ dead_ckind (k+>ec0).
+
+  Proof. auto. Qed.
+
+
+  Lemma dec_context_correct : 
+      forall ec k v, match dec_context ec k v with
+      | in_red r      => ec:[v] = r
+      | in_val v'     => ec:[v] = v'
+      | in_term t ec' => ec:[v] = ec':[t]
+      | in_dead       => dead_ckind (k+>ec)
+      end.
 
   Proof.
-    intros k v ec t H H0.
-    destruct ec, v; inversion H0; subst; 
+    intros ec k v.
+    destruct k, ec; dependent destruction v;
+    simpl;
+    solve [ auto ].
+  Qed.
+
+
+  Lemma dec_context_from_dead : forall ec k v, 
+      dead_ckind (k+>ec) -> dec_context ec k v = in_dead.
+
+  Proof.
+    intros ec k v H.
+    inversion H.
+  Qed.
+
+
+  Lemma dec_context_next_alive : forall ec k v {t ec0}, 
+      dec_context ec k v = in_term t ec0 -> ~ dead_ckind (k+>ec0).
+
+  Proof. auto. Qed.
+
+End MiniML_Strategy.
+
+
+
+
+Module MiniML_Ref_minus <: RED_REF_LANG_minus.
+
+  Module SX := MiniML_PreLang.
+  Module ST := MiniML_Strategy.
+  Module RSF := RED_SYNTAX_Facts SX.
+  Export MiniML_PreLang MiniML_Strategy.
+  Import RSF.
+
+
+
+
+  Module RED_Props.
+
+    Include MiniML_PreLang.
+
+
+    Lemma value_trivial1 : forall {k} (v : value k) ec t, 
+                               ~dead_ckind (k+>ec) -> ec:[t] = v ->
+                                   exists (v' : value (k+>ec)), t = v'.
+
+    Proof.
+      intros k v ec t H H0.
+      destruct ec, v; inversion H0; subst; 
+      eauto.
+    Qed.
+
+
+    Lemma value_redex : forall {k} (v : value k) (r : redex k), 
+                            value_to_term v <> redex_to_term r.
+    Proof.
+      destruct v; destruct r; intro H; discriminate H.
+    Qed.
+
+  End RED_Props.
+
+
+
+
+  Lemma redex_trivial1 : forall {k} (r : redex k) ec t,
+                             ~dead_ckind (k+>ec) -> ec:[t] = r -> 
+                                 exists (v : value (k+>ec)), t = v.
+  Proof with auto.
+    intros k r ec t H H0.
+    destruct ec, r; inversion H0; subst;
     eauto.
   Qed.
-
-
-  Lemma value_redex : forall {k} (v : value k) (r : redex k), 
-                          value_to_term v <> redex_to_term r.
-  Proof.
-    destruct v; destruct r; intro H; discriminate H.
-  Qed.
-
-
-  (*Lemma ot_subterm_val : 
-      forall t t0 ec k, only_trivial t k -> ec:[t0] = t -> 
-          exists v : value k, t0 = v.
-
-  Proof with auto.
-    intros.
-    destruct (H t0 _ (ec0 =: [.])) as [(H1, H2) | (v, H1)]...
-    - discriminateJM H2.
-    - exists v; destruct k...
-  Qed.
-
-
-  Ltac ot_v t ec v0 H0 :=
-      match goal with H : only_trivial ?t0 _ |- _ => unify t0 (ec:[t]);
-          destruct (ot_subterm_val _ t ec _ H) as (v0, H0); [auto | subst t]
-      end.
-
-  Tactic Notation "ot_v" constr(t) constr(ec) "as" ident(v0) ident(H0) := 
-      ot_v t ec v0 H0.
-
-  Ltac mlr rv :=
-      match goal with |- (exists v : value ?k, _ = value_to_term v) \/
-                         (exists r : redex ?k, _ = redex_to_term r)      =>
-          destruct k;
-          match type of rv with
-          | value ?k0 => destruct k0; left;  exists rv
-          | redex ?k0 => destruct k0; right; exists rv
-          end; 
-          simpl; auto
-      end.
-
-
-
-  Lemma trivial_val_red : 
-      forall k t, only_trivial t k ->
-          (exists (v : value k), t = v) \/ (exists (r : redex k), t = r).
-
-  Proof with auto.
-    intros; destruct t.
-    - mlr (vZ : value').
-    - ot_v t s_c as v H0.
-      mlr (vS v : value').
-    - destruct k.
-      ot_v t1 (ap_r t2) as v1 H1.
-      ot_v t2 (ap_l v1) as v2 H2.
-      mlr (rApp v1 v2 : redex').
-    - mlr (vVar v : value').
-    - mlr (vLam v t : value').
-    - ot_v t1 (case_c t2 v t3) as v1 H1.
-      mlr (rCase v1 t2 v t3 : redex').
-    - ot_v t1 (let_c v t2) as v1 H1.
-      mlr (rLet v v1 t2 : redex').
-    - mlr (rFix v t : redex').
-    - destruct k.
-      ot_v t1 (pair_r t2) as v1 H1.
-      ot_v t2 (pair_l v1) as v2 H2.
-      mlr (vPair v1 v2 : value').
-    - ot_v t fst_c as v H0.
-      mlr (rFst v : redex').
-    - ot_v t snd_c as v H0.
-      mlr (rSnd v : redex').
-  Qed.*)
 
 
   Lemma dead_context_dead : 
@@ -332,145 +374,16 @@ Module MiniML_Ref_minus <: RED_REF_LANG_minus.
   Qed.
 
 
-  Lemma proper_death : forall k, dead_ckind k -> ~ exists (r : redex k), True.
-  Proof. auto. Qed.
-
-
-  Module ST <: STRATEGY_STEP SX.
-
-    Inductive interm_dec k : Set :=
-    | in_red  : redex k -> interm_dec k
-    | in_term : term -> elem_context -> interm_dec k
-    | in_val  : value k -> interm_dec k
-    | in_dead : interm_dec k.
-    Arguments in_red {k} _.    Arguments in_val {k} _.
-    Arguments in_term {k} _ _. Arguments in_dead {k}.
-
-    Definition dec_term (t : term) k : interm_dec k :=
-        match t with
-        | Z              =>  in_val vZ
-        | S t            =>  in_term t s_c
-        | App t1 t2      =>  in_term t1 (ap_r t2)
-        | Var x          =>  in_val (vVar x)
-        | Lam x t        =>  in_val (vLam x t)
-        | Case t ez x es =>  in_term t (case_c ez x es)
-        | Letv x t e     =>  in_term t (let_c x e)
-        | Fix x t        =>  in_red (rFix x t)
-        | Pair t1 t2     =>  in_term t1 (pair_r t2)
-        | Fst t          =>  in_term t fst_c
-        | Snd t          =>  in_term t snd_c
-        end.
-
-    Definition dec_context (ec : elem_context) k (v : value (k+>ec)) : interm_dec k :=
-        match ec with
-        | s_c             =>  in_val (vS v)
-        | ap_l v0         =>  in_red (rApp v0 v)
-        | ap_r t          =>  in_term t (ap_l v)
-        | case_c ez x es  =>  in_red (rCase v ez x es)
-        | let_c x e       =>  in_red (rLet x v e)
-        | fst_c           =>  in_red (rFst v)
-        | snd_c           =>  in_red (rSnd v)
-        | pair_l v0       =>  in_val (vPair v0 v)
-        | pair_r t        =>  in_term t (pair_l v)
-        end.
-
-
-    Lemma dec_term_correct : 
-        forall (t : term) k, match dec_term t k with
-        | in_red r      => t = r
-        | in_val v      => t = v
-        | in_term t' ec => t = ec:[t']
-        | in_dead       => dead_ckind k 
-        end.
-
-    Proof with auto.
-      destruct k, t; simpl... 
-    Qed.
-
-
-    Lemma dec_term_from_dead : forall t k, dead_ckind k -> dec_term t k = in_dead.
-    Proof.
-      intros ? k H.
-      inversion H.
-    Qed.
-
-
-    Lemma dec_term_next_alive : 
-        forall t k t0 ec0, dec_term t k = in_term t0 ec0 -> ~ dead_ckind (k+>ec0).
-
-    Proof.
-      auto.
-    Qed.
-
-
-    Lemma dec_context_correct : 
-        forall ec k v, match dec_context ec k v with
-        | in_red r      => ec:[v] = r
-        | in_val v'     => ec:[v] = v'
-        | in_term t ec' => ec:[v] = ec':[t]
-        | in_dead       => dead_ckind (k+>ec)
-        end.
-
-    Proof.
-      intros ec k v.
-      destruct k, ec; dependent destruction v;
-      simpl;
-      solve [ auto ].
-    Qed.
-
-
-    Lemma dec_context_from_dead : forall ec k v, 
-        dead_ckind (k+>ec) -> dec_context ec k v = in_dead.
-
-    Proof.
-      intros ec k v H.
-      inversion H.
-    Qed.
-
-
-    Lemma dec_context_next_alive : forall ec k v {t ec0}, 
-        dec_context ec k v = in_term t ec0 -> ~ dead_ckind (k+>ec0).
-
-    Proof.
-      auto.
-    Qed.
-
-  End ST.
-
-  Export ST.
-
-
-
-  
-  Definition only_empty t k := 
-      forall t' {k'} (c : context k k'), c[t'] = t -> ~ dead_ckind k' -> 
-          k = k' /\ c ~= [.](k).
-
-  Definition only_trivial t k := 
-      forall t' {k'} (c : context k k'),  c[t'] = t -> ~ dead_ckind k' -> 
-          k = k' /\ c ~= [.](k) \/ exists (v : value k'), t' = v.
-
-
-  Lemma redex_trivial1 : forall {k} (r : redex k) ec t,
-                             ~dead_ckind (k+>ec) -> ec:[t] = r -> 
-                                 exists (v : value (k+>ec)), t = v.
-  Proof with auto.
-    intros k r ec t H H0.
-    destruct ec, r; inversion H0; subst;
-    eauto.
-  Qed.
 
 
   Definition subterm_one_step t0 t := exists ec, t = ec:[t0].
 
   Lemma wf_st1 : well_founded subterm_one_step.
-  Proof.
-      RED_REF_LANG_Help.prove_st_wf.
-  Qed.
+  Proof. RED_REF_LANG_Help.prove_st_wf. Qed.
 
 
   Definition subterm_order := clos_trans_1n term subterm_one_step.
-  Notation "a <| b" := (subterm_order a b) (at level 40, no associativity).
+  Notation "t1 <| t2" := (subterm_order t1 t2) (at level 40, no associativity).
   Definition wf_sto : well_founded subterm_order := wf_clos_trans_l _ _ wf_st1.
 
 
@@ -480,13 +393,12 @@ Module MiniML_Ref_minus <: RED_REF_LANG_minus.
       | pair_l _, pair_r _ => immediate_ec ec t /\ immediate_ec ec0 t
       | _, _               => False
       end.
-  Notation "k , t |~  ec1 << ec2 " := (ec_order k t ec1 ec2) (at level 40, no associativity).
+  Notation "k , t |~  ec1 << ec2 " := (ec_order k t ec1 ec2) 
+               (at level 40, no associativity).
 
 
   Lemma wf_eco : forall k t, well_founded (ec_order k t).
-  Proof.
-    RED_REF_LANG_Help.prove_ec_wf.
-  Qed.
+  Proof. RED_REF_LANG_Help.prove_ec_wf. Qed.
 
 
   Lemma ec_order_antisym : forall k t ec ec0, 
@@ -553,6 +465,18 @@ Module MiniML_Ref_minus <: RED_REF_LANG_minus.
   Qed.
 
 
+
+
+  Definition only_empty t k := 
+      forall t' {k'} (c : context k k'), c[t'] = t -> ~ dead_ckind k' -> 
+          k = k' /\ c ~= [.](k).
+
+  Definition only_trivial t k := 
+      forall t' {k'} (c : context k k'),  c[t'] = t -> ~ dead_ckind k' -> 
+          k = k' /\ c ~= [.](k) \/ exists (v : value k'), t' = v.
+
+
+
   Lemma dec_term_red_empty : 
       forall t {k} (r : redex k), dec_term t k = in_red r -> only_empty t k.
 
@@ -570,7 +494,7 @@ Module MiniML_Ref_minus <: RED_REF_LANG_minus.
     - intuition.
     - destruct (IHc _ H) as (H1, H2)...
       dep_subst.
-      destruct ec0; inversion H.
+      solve [ destruct ec0; inversion H ].
   Qed.
 
 
@@ -675,11 +599,27 @@ Module MiniML_Ref_minus <: RED_REF_LANG_minus.
 End MiniML_Ref_minus.
 
 
+
+
 Module MiniML_Ref := mk_RedRefLang MiniML_Ref_minus.
+
+Module MiniML_Extras.
+
+  Import MiniML_Ref.R.
+
+  Notation context'  := (@context () ()).
+  Notation value'    := (@value ()).
+  Notation redex'    := (@redex ()).
+  Notation contract' := (@contract ()).
+  Notation decomp'   := (@decomp ()).
+
+End MiniML_Extras.
+
+
 
 
 Require Import refocusing_semantics_derivation.
 Require Import refocusing_machine.
 
-Module MiniML_REF_SEM := RedRefSem MiniML_Ref.
-Module MiniML_EAM     := ProperEAMachine MiniML_Ref.R MiniML_REF_SEM.
+Module MiniML_RefSem := RedRefSem MiniML_Ref.
+Module MiniML_EAM    := ProperEAMachine MiniML_Ref.R MiniML_RefSem.
