lam_ses_no.v
@@ -1,0 +1,971 @@
+Require Import Util.
+Require Import Program.
+Require Import refocusing_lang.
+Require Import reduction_semantics_facts.
+
+
+
+
+(* Lambda calculus with simple explicit substitution for the normal-order strategy *)
+
+Module Lam_SES_NO_PreLang <: RED_SYNTAX.
+
+  Require Export Peano_dec Compare_dec.
+
+
+  Inductive __term :=
+  | Var   : nat                     -> __term
+  | Lam   : __term                  -> __term
+  | App   : __term -> __term        -> __term
+  | Sub   : __term -> nat -> __term -> __term
+  | Shift : __term -> nat -> nat    -> __term.
+  Definition term := __term.
+
+
+  Inductive substitut := 
+  | st_sub   : term -> substitut 
+  | st_shift : nat -> substitut.
+  Definition sub_tag := (nat * substitut) %type.
+
+
+  Inductive ck := C | ECa | D | CBot.
+  Definition ckind := ck.
+  Hint Unfold ckind.
+
+
+  Definition CECaD (k : ckind) := match k with CBot => False     | _ => True end.
+  Definition CECa  (k : ckind) := match k with CBot | D => False | _ => True end.
+
+  Ltac destruct_all_CECaD :=
+      repeat match goal with H : CECaD ?k |- _ => 
+          try destruct k; destruct H
+      end.
+  Ltac destruct_all_CECa :=
+      repeat match goal with H : CECa ?k |- _ => 
+          try destruct k; destruct H
+      end.
+
+
+  Definition init_ckind : ckind     :=  C.
+  Definition dead_ckind (k : ckind) :=  k = CBot.
+  Hint Unfold init_ckind dead_ckind.
+
+
+  Inductive val : ckind -> Type :=
+
+  | vCLam   : val C -> val C
+  | vCVar   : nat -> val C
+  | vCApp   : valCa -> val C -> val C
+  
+  | vECaLam : term -> val ECa
+  | vECaVar : nat -> val ECa
+  | vECaApp : valCa -> val C -> val ECa
+
+  | vDLam   : term -> val D
+  | vDVar   : nat  -> val D
+  | vDApp   : term -> term -> val D
+  
+  | vCBot   : term -> val CBot
+  
+  with valCa :=
+
+  | vCaVar : nat -> valCa
+  | vCaApp : valCa -> val C -> valCa.
+  
+  Definition value := val.
+  Hint Unfold value.
+
+  Scheme val_Ind   := Induction for val Sort Prop
+    with valCa_Ind := Induction for valCa Sort Prop.
+
+
+  Fixpoint value_to_term {k} (v : value k) : term :=
+      match v with
+      | vCLam v => Lam (value_to_term v)
+      | vCVar x => Var x
+      | vCApp v1 v2 => App (valCa_to_term v1) (value_to_term v2)
+      | vECaLam t => Lam t
+      | vECaVar x => Var x
+      | vECaApp v1 v2 => App (valCa_to_term v1) (value_to_term v2)
+      | vDLam t0 => Lam t0
+      | vDVar n => Var n
+      | vDApp t0 t1 => App t0 t1
+      | vCBot t => t
+      end
+
+  with valCa_to_term v : term :=
+      match v with
+      | vCaVar x => Var x
+      | vCaApp v1 v2 => App (valCa_to_term v1) (value_to_term v2)
+      end.
+
+  Coercion value_to_term : value >-> term.
+  Coercion valCa_to_term : valCa >-> term. 
+
+
+  Definition vVar n k : value k := 
+      match k with 
+      | C => vCVar n | ECa => vECaVar n | D => vDVar n 
+      | CBot => vCBot (Var n) 
+      end.
+
+
+  Inductive red : ckind -> Type :=
+  | rCApp    : term -> term -> red C
+  | rECaApp  : term -> term -> red ECa
+  | rSubVar  : forall k, CECaD k -> nat          -> sub_tag -> red k
+  | rSubLam  : forall k, CECaD k -> term         -> sub_tag -> red k
+  | rSubApp  : forall k, CECaD k -> term -> term -> sub_tag -> red k.
+  Definition redex := red.
+  Hint Unfold redex.
+
+
+  Inductive ec :=
+  | lam_c  : ec
+  | ap_r   : term -> ec
+  | ap_l   : valCa -> ec
+  | stag_c : sub_tag -> ec.
+  Definition elem_context := ec.
+  Hint Unfold elem_context.
+
+
+  Definition elem_plug (t : term) (ec : elem_context) : term :=
+      match ec with
+      | lam_c => Lam t
+      | ap_r tr => App t tr
+      | ap_l v  => App (v : term) t
+      | stag_c (j, st_sub t') => Sub t j t'
+      | stag_c (j, st_shift g) => Shift t j g
+      end.
+  Notation "ec :[ t ]" := (elem_plug t ec) (at level 0).
+
+
+  Definition ckind_trans (k : ckind) (ec : elem_context) := 
+      match k with
+      | C    => match ec with lam_c => C    | ap_r _ => ECa | ap_l _ => C | 
+                              stag_c _ => D end
+      | ECa  => match ec with lam_c => CBot | ap_r _ => ECa | ap_l _ => C | 
+                              stag_c _ => D end
+      | D    => match ec with stag_c _ => D | _ => CBot end
+      | CBot => CBot
+      end.
+  Notation "k +> ec" := (ckind_trans k ec) (at level 50, left associativity).
+
+
+  Inductive context (k1 : ckind) : ckind -> Set :=
+  | empty : context k1 k1
+  | ccons : forall (ec : elem_context) {k2}, context k1 k2 -> context k1 (k2+>ec).
+  Arguments empty {k1}. Arguments ccons {k1} _ {k2} _.
+
+  Notation "[.]"      := empty.
+  Notation "[.]( k )" := (@empty k).
+  Infix "=:"          := ccons (at level 60, right associativity).
+
+
+  Definition redex_to_term {k} (r : redex k) : term :=
+      match r with
+      | rCApp t1 t2   => App (Lam t1) t2
+      | rECaApp t1 t2 => App (Lam t1) t2
+      | rSubVar _ _ n d     => (stag_c d):[Var n]
+      | rSubLam _ _ t d     => (stag_c d):[Lam t]
+      | rSubApp _ _ t1 t2 d => (stag_c d):[App t1 t2]
+      end.
+  Coercion redex_to_term : redex >-> term.
+
+
+
+  Lemma value_to_term_injective : 
+      forall {k} (v v' : value k), value_to_term v = value_to_term v' -> v = v'.
+
+  Proof with auto.
+    induction v using val_Ind with 
+    (P  := fun k v => forall v' : value k, value_to_term v = value_to_term v' -> v = v')
+    (P0 := fun v   => forall v' : valCa,   valCa_to_term v = valCa_to_term v' -> v = v');
+    dependent destruction v'; intro H; inversion H; f_equal...
+  Qed.
+
+
+  Lemma valCa_to_term_injective : 
+      forall v v', valCa_to_term v = valCa_to_term v' -> v = v'.
+
+  Proof with auto.
+    induction v using valCa_Ind with 
+    (P  := fun k v => forall v' : value k, value_to_term v = value_to_term v' -> v = v')
+    (P0 := fun v   => forall v' : valCa,   valCa_to_term v = valCa_to_term v' -> v = v');
+    dependent destruction v'; intro H; inversion H; f_equal...
+  Qed.
+
+
+  Lemma redex_to_term_injective : 
+      forall {k} (r r' : redex k), redex_to_term r = redex_to_term r' -> r = r'.
+
+  Proof with auto.
+    intros k r r' H.
+    destruct k;
+    dependent destruction r; dependent destruction r'; 
+    destruct_all sub_tag; destruct_all substitut; 
+    inversion H; subst;
+
+    solve
+    [ repeat match goal with H : CECaD ?k |- _ => try destruct k; destruct H end;
+      f_equal; auto ].
+  Qed.
+
+
+  Fixpoint compose {k1 k2} (c0 : context k1 k2) 
+                      {k3} (c1 : context k3 k1) : context k3 k2 := 
+      match c0 in context _ k2' return context k3 k2' with
+      | [.]     => c1
+      | ec=:c0' => ec =: compose c0' c1
+      end.
+  Infix "~+" := compose (at level 60, right associativity).
+
+
+  Lemma elem_plug_injective1 : forall ec {t0 t1}, ec:[t0] = ec:[t1] -> t0 = t1.
+
+  Proof.
+    intros ec t0 t1 H.
+    destruct ec;
+    destruct_all sub_tag; destruct_all substitut;
+    solve
+    [ inversion H; trivial ].
+  Qed.
+
+
+  Fixpoint plug t {k1 k2} (c : context k1 k2) : term :=
+      match c with
+      | [.]    => t 
+      | ec=:c' => plug ec:[t] c'
+      end.
+  Notation "c [ t ]" := (plug t c) (at level 0).
+
+
+  Definition immediate_ec ec t := exists t', ec:[t'] = t.
+
+
+  Lemma valCa_is_valECa : 
+      forall v1 : valCa, exists v2 : value ECa, valCa_to_term v1 = value_to_term v2.
+
+  Proof with auto.
+    destruct v1; intros.
+    - exists (vECaVar n)...
+    - exists (vECaApp v1 v)...
+  Qed.
+
+
+  Definition contract0 {k} (r : redex k) : term :=
+      match r with
+      | rCApp   t0 t1 => Sub t0 0 t1
+      | rECaApp t0 t1 => Sub t0 0 t1
+      | rSubVar _ _ i  (j, st_sub t)   => if lt_dec i j     then Var i else 
+                                          if eq_nat_dec i j then Shift t 0 j
+                                                            else Var (pred i)
+      | rSubVar _ _ i  (j, st_shift g) => if lt_dec i j     then Var i
+                                                            else Var (i+g)
+      | rSubLam _ _ t  (j, d)          => Lam ((stag_c (S j, d)):[t])
+      | rSubApp _ _ t1 t2 d            => App (stag_c d):[t1] (stag_c d):[t2]
+      end.
+  Definition contract {k} (r : redex k) := Some (contract0 r).
+
+
+  Lemma death_propagation : 
+      forall k, dead_ckind k -> forall ec, dead_ckind (k+>ec).
+
+  Proof.
+    intros k H.
+    destruct k;
+    inversion H;
+    solve [reflexivity].
+  Qed.
+
+
+  Lemma proper_death : forall k, dead_ckind k -> ~ exists (r : redex k), True.
+
+  Proof with eauto.
+    intros k H [r _].
+    destruct r; inversion H; subst;
+    solve [autof].
+  Qed.
+
+
+End Lam_SES_NO_PreLang.
+
+
+
+
+Module Lam_SES_NO_Strategy <: STRATEGY_STEP Lam_SES_NO_PreLang.
+
+  Import Lam_SES_NO_PreLang.
+
+
+  Inductive interm_dec k : Set :=
+  | in_red  : redex k -> interm_dec k
+  | in_term : term -> elem_context -> interm_dec k
+  | in_val  : value k -> interm_dec k
+  | in_dead : interm_dec k.
+  Arguments in_red {k} _.    Arguments in_val {k} _.
+  Arguments in_term {k} _ _. Arguments in_dead {k}.
+
+
+  Definition dec_term t k : interm_dec k :=
+
+      match k as k0 return interm_dec k0 with 
+      | C    => match t with
+                | App t1 t2 => in_term t1 (ap_r t2)
+                | Var n     => in_val (vCVar n)
+                | Lam t1    => in_term t1 lam_c
+                | Sub t1 n t2   => in_term t1 (stag_c (n, st_sub t2))
+                | Shift t1 n t2 => in_term t1 (stag_c (n, st_shift t2))
+                end
+      | ECa  => match t with
+                | App t1 t2 => in_term t1 (ap_r t2)
+                | Var n     => in_val (vECaVar n)
+                | Lam t1    => in_val (vECaLam t1)
+                | Sub t1 n t2   => in_term t1 (stag_c (n, st_sub t2))
+                | Shift t1 n t2 => in_term t1 (stag_c (n, st_shift t2))
+                end
+      | D    => match t with
+                | App t1 t2 => in_val (vDApp t1 t2)
+                | Var n     => in_val (vDVar n)
+                | Lam t1    => in_val (vDLam t1)
+                | Sub t1 n t2   => in_term t1 (stag_c (n, st_sub t2))
+                | Shift t1 n t2 => in_term t1 (stag_c (n, st_shift t2))
+                end
+      | CBot => in_dead
+      end.
+
+
+  Definition dec_context ec k (v : value (k+>ec)) : interm_dec k :=
+
+      match ec as ec0 return value (k+>ec0) -> interm_dec k with
+
+      | lam_c    => match k as k0 return value (k0+>lam_c) -> interm_dec k0 with
+                    | C    => fun v => in_val (vCLam v)
+                    | ECa  => fun _ => in_dead
+                    | D    => fun _ => in_dead
+                    | CBot => fun _ => in_dead
+                    end
+
+      | ap_r t   => match k as k0 return value (k0+>(ap_r t)) -> interm_dec k0 with
+                    | C    => fun v => 
+                                  match v with
+                                  | vECaLam t0    => in_red (rCApp t0 t)
+                                  | vECaVar n     => in_term t (ap_l (vCaVar n))
+                                  | vECaApp v1 v2 => in_term t (ap_l (vCaApp v1 v2))
+                                  | _ => @in_dead C
+                                  end
+                    | ECa  => fun v => 
+                                  match v with
+                                  | vECaLam t0    => in_red (rECaApp t0 t)
+                                  | vECaVar n     => in_term t (ap_l (vCaVar n))
+                                  | vECaApp v1 v2 => in_term t (ap_l (vCaApp v1 v2))
+                                  | _ => @in_dead ECa
+                                  end
+                    | D    => fun _ => in_dead
+                    | CBot => fun _ => in_dead
+                    end
+
+      | ap_l v0  => match k as k0 return value (k0+>(ap_l v0)) -> interm_dec k0 with
+                    | C    => fun v => in_val (vCApp v0 v)
+                    | ECa  => fun v => in_val (vECaApp v0 v)
+                    | D    => fun _ => in_dead
+                    | CBot => fun _ => in_dead
+                    end
+
+      | stag_c d => match k as k0 return value (k0+>(stag_c d)) -> interm_dec k0 with
+                    | CBot => fun _ => in_dead
+                    | k0   => fun v => 
+                                  match v with
+                                  | vDLam t0    => in_red (rSubLam k0 I t0 d)
+                                  | vDVar n     => in_red (rSubVar k0 I n  d)
+                                  | vDApp t1 t2 => in_red (rSubApp k0 I t1 t2 d)
+                                  | _ => @in_dead k0
+                                  end
+                    end
+      end v.
+
+
+  Lemma dec_term_correct : 
+      forall (t : term) k, match dec_term t k with
+      | in_red r      => t = r
+      | in_val v      => t = v
+      | in_term t' ec => t = ec:[t']
+      | in_dead       => dead_ckind k 
+      end.
+
+  Proof.
+    destruct k, t; simpl; 
+    auto.
+  Qed.
+
+
+  Lemma dec_term_from_dead : forall t k, dead_ckind k -> dec_term t k = in_dead.
+  Proof.
+    intros t k H.
+    destruct k;
+    solve [ autof ].
+  Qed.
+
+
+  Lemma dec_term_next_alive : 
+      forall t k t0 ec0, dec_term t k = in_term t0 ec0 -> ~ dead_ckind (k+>ec0).
+
+  Proof.
+    intros t k t0 ec0 H.
+    destruct t, k;
+    solve [ inversion H; subst; 
+            auto ].
+  Qed.
+
+
+  Lemma dec_context_correct : 
+      forall ec k v, match dec_context ec k v with
+      | in_red r      => ec:[v] = r
+      | in_val v'     => ec:[v] = v'
+      | in_term t ec' => ec:[v] = ec':[t]
+      | in_dead       => dead_ckind (k+>ec)
+      end.
+
+  Proof.
+    intros ec k v.
+    destruct k, ec; dependent destruction v;
+    simpl;
+    solve [ auto ].
+  Qed.
+
+
+  Lemma dec_context_from_dead : forall ec k v, 
+      dead_ckind (k+>ec) -> dec_context ec k v = in_dead.
+
+  Proof.
+    intros ec k v H.
+    destruct ec, k;
+    solve [ autof ].
+  Qed.
+
+
+  Lemma dec_context_next_alive : forall ec k v {t ec0}, 
+      dec_context ec k v = in_term t ec0 -> ~ dead_ckind (k+>ec0).
+
+  Proof.
+    intros ec k v t ec0 H.
+    destruct ec, ec0, k; dependent destruction v;  
+    solve [ autof ].
+  Qed.
+
+End Lam_SES_NO_Strategy.
+
+
+
+
+Module Lam_SES_NO_Ref_minus <: RED_REF_LANG_minus.
+
+  Module SX := Lam_SES_NO_PreLang.
+  Module ST := Lam_SES_NO_Strategy.
+  Module SXF := RED_SYNTAX_Facts SX.
+  Export Lam_SES_NO_PreLang Lam_SES_NO_Strategy.
+  Import SXF.
+
+
+
+  Module RED_Props.
+
+    Include Lam_SES_NO_PreLang.
+
+    Lemma value_trivial1 : forall {k} (v : value k) ec t, 
+                               ~dead_ckind (k+>ec) -> ec:[t] = v ->
+                                   exists (v' : value (k+>ec)), t = v'.
+    Proof.
+      intros k v ec t H H0.
+      destruct ec, v; destruct_all sub_tag; destruct_all substitut; 
+      inversion H0; subst;
+      solve
+      [ eautof
+      | auto using valCa_is_valECa ].
+    Qed.
+
+
+    Lemma value_redex : forall {k} (v : value k) (r : redex k), 
+                            value_to_term v <> redex_to_term r.
+    Proof.
+      intros k v r.
+
+      dependent destruction r; dependent destruction v; 
+      simpl;
+      try match goal with 
+      | |- App (valCa_to_term ?v) _ <> _ => dependent_destruction2 v
+      end;
+      destruct_all sub_tag; destruct_all substitut;
+      
+      solve [ discriminate | tauto ].
+    Qed.
+
+  End RED_Props.
+
+
+
+
+  Lemma dead_context_dead : 
+      forall {k1 k2}, context k1 k2 -> dead_ckind k1 -> dead_ckind k2.
+
+  Proof with auto.
+    intros ? ? c H; revert c.
+    induction 1.
+    - trivial.
+    - apply death_propagation...
+  Qed.
+
+
+  Lemma redex_trivial1 : forall {k} (r : redex k) ec t,
+                             ~dead_ckind (k+>ec) -> ec:[t] = r -> 
+                                 exists (v : value (k+>ec)), t = v.
+  Proof.
+    intros k r ec t H H0.
+    destruct ec, r; destruct_all sub_tag; destruct_all substitut; destruct_all_CECaD;
+    inversion H0; subst;
+    try solve 
+    [ eexists (vECaLam _); simpl; eauto
+    | eexists (vCLam _); simpl; eauto
+    | eexists (vDLam _); simpl; eauto
+    | eexists (vECaApp _ _); simpl; eauto
+    | eexists (vCApp _ _); simpl; eauto
+    | eexists (vDApp _ _); simpl; eauto
+    | eexists (vECaVar _); simpl; eauto
+    | eexists (vCVar _); simpl; eauto
+    | eexists (vDVar _); simpl; eauto
+    | match goal with v: valCa |- _ => destruct v; discriminate end ].
+  Qed.
+
+
+
+
+  Definition subterm_one_step t0 t := exists ec, t = ec:[t0].
+  Lemma wf_st1 : well_founded subterm_one_step.
+  Proof.
+    RED_REF_LANG_Help.prove_st_wf;
+
+    solve
+    [ destruct_all sub_tag; destruct_all substitut;
+      inversion H1; subst; 
+      auto ].
+  Qed.
+
+
+  Definition subterm_order := clos_trans_1n term subterm_one_step.
+  Notation "t1 <| t2" := (subterm_order t1 t2) (at level 70, no associativity).
+  Definition wf_sto : well_founded subterm_order := wf_clos_trans_l _ _ wf_st1.
+
+
+  Definition ec_order (k : ckind) (t : term) (ec ec0 : elem_context) : Prop :=
+      match k with
+      | CBot | D => False
+      | _        => match ec, ec0 with 
+                    | ap_l _, ap_r _ => immediate_ec ec t /\ immediate_ec ec0 t 
+                    | _, _           => False
+                    end
+      end.
+  Notation "k , t |~  ec1 << ec2 " := (ec_order k t ec1 ec2) 
+               (at level 70, t, ec1, ec2 at level 50, no associativity).
+
+
+  Lemma wf_eco : forall k t, well_founded (ec_order k t).
+  Proof. RED_REF_LANG_Help.prove_ec_wf. Qed.
+
+
+  Lemma ec_order_antisym : forall k t ec ec0, 
+      k, t |~ ec << ec0 -> ~ k, t |~ ec0 << ec.
+
+  Proof.
+    intros k t ec ec0 H.
+    destruct k, ec, ec0;
+    solve [ autof ].
+  Qed.
+
+
+  Lemma ec_order_trans :  forall k t ec0 ec1 ec2, 
+      k,t |~ ec0 << ec1 -> k,t |~ ec1 << ec2 -> 
+      k,t |~ ec0 << ec2.
+
+  Proof.
+    intros k t ec0 ec1 ec2 H H0.
+    destruct k, ec0, ec1;
+    solve [ autof ].
+  Qed.
+
+
+  Lemma ec_order_comp_if : forall t ec0 ec1, 
+      immediate_ec ec0 t -> immediate_ec ec1 t -> 
+      forall k, ~ dead_ckind (k+>ec0) -> ~ dead_ckind (k+>ec1) ->
+          k,t |~ ec0 << ec1 \/ k,t |~ ec1 << ec0 \/ ec0 = ec1.
+
+  Proof.
+    intros t ec0 ec1 H0 H1 k H2 H3.
+
+    destruct H0 as (t0, H4); destruct H1 as (t1, H5).
+    subst t.
+    destruct k, ec0, ec1;
+    destruct_all sub_tag; destruct_all substitut;
+    inversion H5; subst;
+
+    solve
+    [ compute; eautof 7
+    | do 2 right; 
+      f_equal;
+      apply valCa_to_term_injective; auto ].
+  Qed.
+
+
+  Lemma ec_order_comp_fi :
+      forall k t ec0 ec1,  k, t |~ ec0 << ec1 ->
+          immediate_ec ec0 t /\ immediate_ec ec1 t /\ 
+          ~ dead_ckind (k+>ec0) /\ ~ dead_ckind (k+>ec1).
+
+  Proof with auto.
+    intros k t ec0 ec1 H.
+    destruct k, ec0, ec1;
+    destruct_all sub_tag; destruct_all substitut;
+    inversion H;
+    solve [auto].
+  Qed.
+
+
+  Lemma death_propagation2 : 
+      forall k ec, ~ dead_ckind (k+>ec) -> ~ dead_ckind k.
+
+  Proof.
+    intuition.
+    apply H.
+    apply death_propagation.
+    assumption.
+  Qed.
+
+
+
+
+  Definition only_empty t k := 
+      forall t' {k'} (c : context k k'), c[t'] = t -> ~ dead_ckind k' -> 
+          k = k' /\ c ~= [.](k).
+
+  Definition only_trivial t k := 
+      forall t' {k'} (c : context k k'),  c[t'] = t -> ~ dead_ckind k' -> 
+          k = k' /\ c ~= [.](k) \/ exists (v : value k'), t' = v.
+
+
+  Lemma dec_term_red_empty : 
+      forall t k (r : redex k), dec_term t k = in_red r -> only_empty t k.
+
+  Proof with auto.
+    intros t k r H.
+    destruct t; 
+    inversion H; subst; clear H;
+
+    solve
+    [ intros t0 k' c H H0; generalize dependent t0;
+
+      induction c;
+      intros; simpl in *;
+      [ intuition
+      | destruct (IHc (death_propagation2 _ _ H0) _ H);
+        dep_subst;
+        destruct k2, ec0;
+        solve [inversion H1; auto] 
+    ] ].
+  Qed.
+
+
+  Lemma dec_term_val_empty : forall t k (v : value k), 
+                                 dec_term t k = in_val v -> only_empty t k.
+  Proof with auto.
+    intros t k v H.
+    destruct t;
+    intros t0 k' c H0 H1; generalize dependent t0;
+    solve
+    [ induction c;
+      intros t0 H0; simpl in *;
+      [ intuition
+      | destruct (IHc (death_propagation2 _ _ H1) _ H0); dep_subst;
+        simpl in H;
+        destruct k2, ec0; 
+        destruct_all sub_tag; destruct_all substitut;
+        inversion H; subst; 
+        solve [discriminate H | autof] 
+    ] ].
+  Qed.
+
+
+  Lemma dec_term_term_top : forall t k {t' ec}, 
+            dec_term t k = in_term t' ec -> forall ec', ~ k, t |~ ec << ec'.
+
+  Proof.
+    intros t k t' ec H ec' H0.
+    destruct k, t, ec'; 
+    solve [ inversion H; subst; inversion H0 ].
+  Qed.
+
+
+  Lemma dec_context_red_bot : 
+      forall k ec v r, dec_context ec k v = in_red r -> 
+          forall ec', ~ k, ec:[v] |~ ec' << ec.
+  Proof.
+    intros k ec v r H ec'.
+    destruct k, ec, ec'; dependent destruction v;
+    solve
+    [ autof
+    | inversion H;
+      intro G;
+      unfold ec_order in G; destruct G as (G, _);
+      destruct G as (t1, G); inversion G; subst;
+      destruct v0; 
+      autof ].
+  Qed.
+
+
+  Lemma dec_context_val_bot : 
+      forall k ec v v', dec_context ec k v = in_val v' -> 
+          forall ec', ~ k, ec:[v] |~ ec' << ec.
+  Proof.
+    intros k ec v v' H ec'.
+    destruct k, ec, ec'; dependent destruction v; 
+    solve [ autof ].
+  Qed.
+
+
+  Lemma dec_context_term_next : 
+      forall ec0 k v t ec1, dec_context ec0 k v = in_term t ec1 ->
+      (*1*) k, ec0:[v] |~ ec1 << ec0 /\ 
+      (*2*) forall ec,  k, ec0:[v] |~ ec << ec0  ->  ~ k, ec0:[v] |~ ec1 << ec.
+
+  Proof.
+    intros ec0 k v t ec1 H.
+    destruct k, ec0, ec1; dependent destruction v; 
+    solve 
+    [ autof
+
+    | inversion H; subst;
+      split;
+      [ constructor; 
+        compute; eauto
+      | intros ec'' H0 H1; 
+        destruct ec'';
+        solve [ autof ] 
+      ] ].
+  Qed.
+
+
+  Lemma elem_context_det : 
+      forall t ec {t'}, t = ec:[t'] -> 
+          forall k ec',  k, t |~ ec' << ec -> 
+              exists (v : value (k+>ec)), t' = v.
+
+  Proof.
+    intros t ec0 t' H k ec' H0.
+    subst.
+
+    destruct k, ec0, ec'; autof;
+    unfold ec_order in H0; destruct H0 as (H, _);
+    destruct (valCa_is_valECa v) as (v0, H0);
+
+    solve
+    [ exists v0;
+      simpl; rewrite <- H0;
+      inversion H as (t0, H1); inversion H1; 
+      trivial ].
+  Qed.
+
+End Lam_SES_NO_Ref_minus.
+
+
+
+Module Lam_SES_NO_Ref := mk_RedRefLang Lam_SES_NO_Ref_minus.
+
+
+
+
+(* Contexts from the Johan Munk's paper *)
+
+Module Lam_SES_NO_AlterContexts.
+
+  Import Lam_SES_NO_PreLang.
+
+  Inductive ckind_IO := Aio | Cio | Dio.
+
+  Inductive context_IO : ckind_IO -> Set :=
+  | hole_io   : context_IO Aio
+  | ap_l_io   : context_IO Cio -> valCa -> context_IO Aio
+  | lam_c_io  : context_IO Aio -> context_IO Aio
+
+  | a_is_c_io : context_IO Aio -> context_IO Cio
+  | ap_r_io   : context_IO Cio -> term -> context_IO Cio
+
+  | c_is_d_io : context_IO Cio -> context_IO Dio
+  | stag_c_io : context_IO Dio -> sub_tag -> context_IO Dio.
+
+  Definition a_is_d_io c := c_is_d_io (a_is_c_io c).
+
+
+  Definition context_to_IO {k1 k2} (c : context k1 k2) : 
+               match k2 with  
+               | C => context_IO Aio | ECa => context_IO Cio 
+               | D => context_IO Dio | CBot => unit
+               end.
+
+    induction c as  [ | ec k2 c IHc].
+    
+    (* c = [.] *)
+    - destruct k1.
+      + exact hole_io.
+      + exact (a_is_c_io hole_io).
+      + exact (a_is_d_io hole_io).
+      + exact ().
+    
+    (* c = (ec=:c') *)
+    - set (e:=ec).
+      destruct k2, ec; simpl;
+      match goal with
+      | e := lam_c                           |- _ => exact (lam_c_io IHc)
+      | e := ap_r ?t, IHc : context_IO Aio   |- _ => exact (ap_r_io (a_is_c_io IHc) t)
+      | e := ap_r ?t, IHc : context_IO Cio   |- _ => exact (ap_r_io IHc t)
+      | e := ap_l ?v, IHc : context_IO Aio   |- _ => exact (ap_l_io (a_is_c_io IHc) v)
+      | e := ap_l ?v, IHc : context_IO Cio   |- _ => exact (ap_l_io IHc v)
+      | e := stag_c ?d, IHc : context_IO Aio |- _ => exact (stag_c_io (a_is_d_io IHc) d)
+      | e := stag_c ?d, IHc : context_IO Cio |- _ => exact (stag_c_io (c_is_d_io IHc) d)
+      | e := stag_c ?d, IHc : context_IO Dio |- _ => exact (stag_c_io IHc d)
+      | _                                         => exact ()
+      end.
+  Defined.
+
+
+  Definition context_from_IO {k} (c : context_IO k) : 
+               match k with  
+               | Aio => context C C | Cio => context C C + context C ECa 
+               | Dio => context C C + context C ECa + context C D
+               end.
+
+    set (c0:=c).
+    induction c as [ | ? IHc ? | ? IHc | ? IHc | ? IHc ? | ? IHc | ? IHc ?]; simpl in *;
+    match goal with
+    | c0 := hole_io        |- _ => exact [.]
+    | c0 := ap_l_io _ ?v   |- _ => destruct IHc as [IHc | IHc];
+                                   exact (ap_l v=:IHc)
+    | c0 := lam_c_io _     |- _ => exact (lam_c=:IHc)
+    | c0 := a_is_c_io _    |- _ => exact (inl IHc)
+    | c0 := ap_r_io _ ?t   |- _ => destruct IHc as [IHc | IHc];
+                                   exact (inr (ap_r t=:IHc))
+    | c0 := c_is_d_io _    |- _ => exact (inl IHc)
+    | c0 := stag_c_io _ ?d |- _ => destruct IHc as [[IHc | IHc] | IHc];
+                                   exact (inr (stag_c d=:IHc))
+    end.
+  Defined.
+
+
+  Lemma to_from_IO_is_id : 
+            forall k (c : context_IO k),
+                match k as k return context_IO k -> Prop with
+                | Cio => fun c =>
+                    c = match context_from_IO c with 
+                        | inl c => a_is_c_io (context_to_IO c) 
+                        | inr c => context_to_IO c 
+                        end
+                | Aio => fun c => c = context_to_IO (context_from_IO c)
+                | Dio => fun c =>
+                    c = match context_from_IO c with 
+                        | inl (inl c) => a_is_d_io (context_to_IO c) 
+                        | inl (inr c) => c_is_d_io (context_to_IO c) 
+                        | inr c => context_to_IO c 
+                        end
+                end c.
+  Proof.
+    induction c; 
+        simpl;
+        repeat match goal with
+        | _ : context [match ?s with inl _ => _ | inr _ => _ end] |- _ => destruct s
+        end;
+        try subst;
+    solve
+    [ simpl; f_equal; auto ].
+  Qed.
+
+
+  Lemma from_to_IO_is_id : 
+            forall k (c : context C k),
+                match k as k return context C k -> Prop with
+                | C    => fun c =>     c = context_from_IO (context_to_IO c)
+                | ECa  => fun c => inr c = context_from_IO (context_to_IO c)
+                | D    => fun c => inr c = context_from_IO (context_to_IO c)
+                | CBot => fun c => True
+                end c.
+  Proof.
+    induction c as [ | ec k2 ? IHc].
+    - simpl; auto.
+    - destruct k2, ec; 
+      simpl; 
+      try rewrite <- IHc; 
+      solve [congruence | auto].
+  Qed.
+
+
+  Fixpoint plug_IO t {k} (c : context_IO k) :=
+      match c with
+      | hole_io       => t
+      | ap_l_io c' v  => plug_IO (App (v : term) t) c'
+      | lam_c_io c'   => plug_IO (Lam t) c'
+      | a_is_c_io c'  => plug_IO t c'
+      | ap_r_io c' t' => plug_IO (App t t') c'
+      | c_is_d_io c'  => plug_IO t c'
+      | stag_c_io c' (n, st_sub t')  => plug_IO (Sub t n t') c'
+      | stag_c_io c' (n, st_shift m) => plug_IO (Shift t n m) c'
+      end.
+
+
+  Lemma plug_compatible : 
+          forall {k1 k2} (c : context k1 k2) t,
+              match k2 as k2 return context k1 k2 -> Prop with
+              | CBot => fun _ => True
+              | k2   => fun c => c[t] = plug_IO t (context_to_IO c) 
+              end c.
+  Proof.
+    induction c.
+    - destruct k1; auto.
+    - destruct k2, ec0; 
+      destruct_all sub_tag; destruct_all substitut; 
+      solve [simpl in *; auto].
+  Qed.
+
+
+  Lemma plug_compatible2 : 
+          forall {k} (c : context_IO k) (t : term),
+              plug_IO t c =
+              match k as k return context_IO k -> term with
+              | Aio => fun c => (context_from_IO c)[t]
+              | Cio => fun c => match context_from_IO c with 
+                                | inl c | inr c => c[t] end
+              | Dio => fun c => match context_from_IO c with 
+                                | inl (inl c) | inl (inr c) | inr c => c[t] end
+              end c.
+  Proof.
+    intros k c t.
+    symmetry.
+    destruct k;
+        first
+        [ rewrite (to_from_IO_is_id Aio) at 2
+        | rewrite (to_from_IO_is_id Cio) at 2
+        | rewrite (to_from_IO_is_id Dio) at 2 ];
+        repeat match goal with
+        | |- context [match ?s with inl _ => _ | inr _ => _ end] => destruct s
+        end;
+    solve
+    [ apply @plug_compatible with (k2 := C)
+    | apply @plug_compatible with (k2 := ECa)
+    | apply @plug_compatible with (k2 := D) ].
+  Qed.
+
+End Lam_SES_NO_AlterContexts.
+
+
+
+
+Require Import refocusing_semantics_derivation.
+Require Import refocusing_machine.
+
+Module Lam_SES_NO_RefSem := RedRefSem Lam_SES_NO_Ref.
+Module Lam_SES_NO_EAM    := ProperEAMachine Lam_SES_NO_Ref.R Lam_SES_NO_RefSem.
